proved that SimpleSE.dbop <-> LLVMopsem.dbop, which completed the proof that TV is correct wrt LLVMopsem.
Problem to fix: 
1) opsem doesn't need to carry the 'block' under execution, the label of that block is enough, otherwise it makes some lemmas hard to prove.
2) functions that look up fdefs and blocks also need to redefine.



git-svn-id: https://webdav.seas.upenn.edu/svn/sol/vol@2540 eef5ea85-cc2e-0410-bd84-0fae1f012da8

src/TV/symexe_correct.v
@@ -15,32 +15,11 @@ Require Import trace.
 Require Import symexe_def.
 Require Import symexe_complete.
 Require Import symexe_sound.
+Require Import seop_llvmop.
 
 Export SimpleSE.
 
-(* Correctness of the cmds validator *)
-
-Definition tv_cmds (nbs1 nbs2 : list nbranch) (lc gl:GVMap) :=
-se_cmds (mkSstate (env_to_smap gl lc) smem_init sframe_init nil) nbs1 =
-se_cmds (mkSstate (env_to_smap gl lc) smem_init sframe_init nil) nbs2.
-
-Lemma tv_cmds__is__correct : forall TD nbs nbs' lc1 als1 gl1 Mem1 lc2 als2 gl2 Mem2 tr,
-  uniq gl1 ->
-  uniq lc1 ->  
-  wf_nbranchs nbs' ->
-  tv_cmds nbs nbs' lc1 gl1 ->
-  dbCmds TD lc1 als1 gl1 Mem1 (nbranchs2cmds nbs) lc2 als2 gl2 Mem2 tr ->
-  dbCmds TD lc1 als1 gl1 Mem1 (nbranchs2cmds nbs') lc2 als2 gl2 Mem2 tr.
-Proof.
-  intros TD nbs nbs' lc1 als1 gl1 Mem1 lc2 als2 gl2 Mem2 tr Huniqg Huniqc Wf Htv_cmds HdbCmds.
-  unfold tv_cmds in Htv_cmds.
-  assert (Uniqs:=HdbCmds).
-  apply dbCmds_uniq in Uniqs; auto.
-  destruct Uniqs as [Uniqg2 Uniqc2].
-  apply op_cmds__satisfy__se_cmds in HdbCmds; auto.
-  rewrite Htv_cmds in HdbCmds.
-  apply se_cmds__denote__op_cmds; auto.
-Qed.
+(* cmd2sbs *)
 
 Record subblock := mkSB
 {
@@ -49,29 +28,6 @@ Record subblock := mkSB
   call_cmd_isCall : Instruction.isCallInst call_cmd = true
 }.
 
-Definition tv_subblock (sb1 sb2:subblock) (lc gl:GVMap) :=
-match (sb1, sb2) with
-| (mkSB nbs1 call1 iscall1, mkSB nbs2 call2 iscall2) =>
-  let st1 := se_cmds (mkSstate (env_to_smap gl lc) smem_init sframe_init nil) nbs1 in
-  let st2 := se_cmds (mkSstate (env_to_smap gl lc) smem_init sframe_init nil) nbs2 in
-  let cl1 := se_call st1 call1 iscall1 in
-  let cl2 := se_call st2 call2 iscall2 in
-  st1 = st2 /\ call1 = call2
-end.
-
-Fixpoint tv_subblocks (sbs1 sbs2:list subblock) (lc gl:GVMap) :=
-match (sbs1, sbs2) with
-| (nil, nil) => True
-| (sb1::sbs1', sb2::sbs2') => tv_subblock sb1 sb2 lc gl /\ tv_subblocks sbs1' sbs2' lc gl 
-| _ => False
-end.
-
-Fixpoint tv_phinodes (ps1 ps2:list phinode) :=
-match (ps1, ps2) with
-| (nil, nil) => True
-| (p1::ps1', p2::ps2') => p1=p2 /\ tv_phinodes ps1' ps2'
-| _ => False
-end.
 
 Fixpoint cmds2sbs (cs:list cmd) : (list subblock*list nbranch) :=
 match cs with
@@ -91,205 +47,6 @@ match cs with
   end
 end.
 
-Definition tv_block (b1 b2:block) (lc gl:GVMap) :=
-match (b1, b2) with
-| (block_intro l1 ps1 cs1 tmn1, block_intro l2 ps2 cs2 tmn2) =>
-  match (cmds2sbs cs1, cmds2sbs cs2) with
-  | ((sbs1, nbs1), (sbs2, nbs2)) =>
-    l1 = l2 /\ 
-    tv_phinodes ps1 ps2 /\ 
-    tv_subblocks sbs1 sbs2 lc gl /\ 
-    tv_cmds nbs1 nbs2 lc gl /\ 
-    tmn1 = tmn2
-  end
-end.
-
-Fixpoint tv_blocks (bs1 bs2:list block) (lc gl:GVMap) :=
-match (bs1, bs2) with
-| (nil, nil) => True
-| (b1::bs1', b2::bs2') => tv_block b1 b2 lc gl /\ tv_blocks bs1' bs2' lc gl 
-| _ => False
-end.
-
-Variable lc0 gl0 : GVMap.
-
-Definition tv_fdef (f1 f2:fdef) (gl:GVMap) :=
-match (f1, f2) with
-| (fdef_intro fh1 lb1, fdef_intro fh2 lb2) =>
-  fh1 = fh2 /\ tv_blocks lb1 lb2 lc0 gl
-end.
-
-Fixpoint tv_products (Ps1 Ps2:list product):=
-match (Ps1, Ps2) with
-| (nil, nil) => True
-| (product_fdec f1::Ps1', product_fdec f2::Ps2') => 
-  f1 = f2 /\ tv_products Ps1' Ps2'
-| (product_fdef f1::Ps1', product_fdef f2::Ps2') => 
-  tv_fdef f1 f2 gl0 /\ tv_products Ps1' Ps2'
-| (product_gvar gvar1::Ps1', product_gvar gvar2::Ps2') => 
-  gvar1 = gvar2 /\ tv_products Ps1' Ps2'
-| _ => False
-end.
-
-Definition tv_module (m1 m2:module) :=
-match (m1, m2) with
-| (module_intro TD1 Ps1, module_intro TD2 Ps2) =>
-  TD1 = TD2 /\ tv_products Ps1 Ps2
-end.
-
-Fixpoint tv_system (S1 S2:system) :=
-match (S1, S2) with
-| (nil, nil) => True
-| (m1::S1', m2::S2') => tv_module m1 m2 /\ tv_system S1' S2'
-| _ => False
-end.
-
-Inductive wf_subblock : subblock -> Prop :=
-| wf_subblock_intro : forall nbs call0 iscall0, 
-  wf_nbranchs nbs ->
-  wf_subblock (mkSB nbs call0 iscall0).
-
-Inductive wf_subblocks : list subblock -> Prop :=
-| wf_subblocks_nil : wf_subblocks nil
-| wf_subblocks_cons : forall sb sbs,
-  wf_subblock sb ->
-  wf_subblocks sbs ->
-  wf_subblocks (sb::sbs).
-
-Inductive wf_block : block -> Prop :=
-| wf_block_intro : forall l ps cs sbs nbs tmn, 
-  cmds2sbs cs = (sbs,nbs) ->
-  wf_subblocks sbs ->
-  wf_nbranchs nbs ->
-  wf_block (block_intro l ps cs tmn).
-
-Lemma tv_terminator__is__correct : forall TD fh1 lb1 fh2 lb2 B1 B2 lc gl tmn B1' lc' tr,
-  tv_fdef (fdef_intro fh1 lb1) (fdef_intro fh2 lb2) gl0 ->
-  tv_block B1 B2 lc gl ->
-  dbTerminator TD (fdef_intro fh1 lb1) B1 lc gl tmn B1' lc' tr ->
-  exists B2', exists n,
-    tv_block B1' B2' lc gl /\
-    nth_error lb1 n = Some B1' /\
-    nth_error lb2 n = Some B2' /\
-    dbTerminator TD (fdef_intro fh2 lb2) B2 lc gl tmn B2' lc' tr.
-Proof.
-  intros TD fh1 lb1 fh2 lb2 B1 B2 lc gl tmn B1' lc' tr Htv_fdef Htv_block HdbTerminator.
-  inversion HdbTerminator; subst.
-    assert (exists B2', exists n, tv_block (block_intro l' ps' sbs' tmn') B2' lc gl /\ 
-                                  nth_error lb1 n = Some (block_intro l' ps' sbs' tmn') /\
-                                  nth_error lb2 n = Some B2') as J.
-      admit. (*lookup*)
-    destruct J as [B2' [n [J1 [J2 J3]]]].
-    exists B2'. exists n. split; auto. split; auto. split; auto.
-    destruct B2' as [l2' ps2' sbs2' tmn2'].
-    apply dbBranch with (c:=c); auto.
-      admit. (*lookup*)
-      admit. (*switch*)
-    
-    assert (exists B2', exists n, tv_block (block_intro l' ps' sbs' tmn') B2' lc gl /\ 
-                                  nth_error lb1 n = Some (block_intro l' ps' sbs' tmn') /\
-                                  nth_error lb2 n = Some B2') as J.
-      admit. (*lookup*)
-    destruct J as [B2' [n [J1 [J2 J3]]]].
-    exists B2'. exists n. split; auto. split; auto. split; auto.
-    destruct B2' as [l2' ps2' sbs2' tmn2'].
-    apply dbBranch_uncond; auto.
-      admit. (*lookup*)
-      admit. (*switch*)
-Qed.
-
-Definition tv_dbCall__is__correct_prop S1 TD Ps1 lc gl Mem0 call0 lc' gl' Mem' tr
-  (db:dbCall S1 TD Ps1 lc gl Mem0 call0 lc' gl' Mem' tr) :=
-  forall S2 Ps2,
-  tv_system S1 S2 ->
-  tv_products Ps1 Ps2 ->
-  dbCall S2 TD Ps2 lc gl Mem0 call0 lc' gl' Mem' tr.
-Definition tv_subblock__is__correct_prop S1 TD Ps1 lc als gl Mem cs1 lc' als' gl' Mem' tr
-  (db:dbSubblock S1 TD Ps1 lc als gl Mem cs1 lc' als' gl' Mem' tr) :=
-  forall S2 Ps2 cs2 sb1 sb2,
-  uniq gl ->
-  uniq lc ->
-  cmds2sbs cs1 = (sb1::nil, nil) ->
-  cmds2sbs cs2 = (sb2::nil, nil) ->
-  wf_subblock sb2 ->
-  tv_system S1 S2 ->
-  tv_products Ps1 Ps2 ->
-  tv_subblock sb1 sb2 lc gl ->
-  dbSubblock S2 TD Ps2 lc als gl Mem cs2 lc' als' gl' Mem' tr.
-Definition tv_subblocks__is__correct_prop S1 TD Ps1 lc als gl Mem cs1 lc' als' gl' Mem' tr
-  (db:dbSubblocks S1 TD Ps1 lc als gl Mem cs1 lc' als' gl' Mem' tr) :=
-  forall S2 Ps2 sbs1 sbs2 cs2,
-  uniq gl ->
-  uniq lc ->
-  cmds2sbs cs1 = (sbs1, nil) ->
-  cmds2sbs cs2 = (sbs2, nil) ->
-  wf_subblocks sbs2 ->
-  tv_system S1 S2 ->
-  tv_products Ps1 Ps2 ->
-  tv_subblocks sbs1 sbs2 lc gl ->
-  dbSubblocks S2 TD Ps2 lc als gl Mem cs2 lc' als' gl' Mem' tr.
-Definition tv_block__is__correct_prop S1 TD Ps1 F1 arg state1 state2 tr
-  (db:dbBlock S1 TD Ps1 F1 arg state1 state2 tr) :=
-  forall S2 Ps2 fh1 lb1 fh2 lb2 B1 lc als gl Mem B1' lc' als' gl' Mem' B2,
-  state1 = mkState (mkEC B1 lc als) gl Mem ->
-  state2 = mkState (mkEC B1' lc' als') gl' Mem' ->
-  F1 = fdef_intro fh1 lb1 ->
-  uniq gl ->
-  uniq lc ->
-  wf_block B2 ->
-  tv_system S1 S2 ->
-  tv_products Ps1 Ps2 ->
-  tv_fdef (fdef_intro fh1 lb1) (fdef_intro fh2 lb2) gl0 ->
-  tv_block B1 B2 lc gl ->
-  exists B2', exists n,
-    dbBlock S2 TD Ps2 (fdef_intro fh2 lb2) arg 
-      (mkState (mkEC B2 lc als) gl Mem) 
-      (mkState (mkEC B2' lc' als') gl' Mem')
-      tr /\
-    nth_error lb1 n = Some B1' /\
-    nth_error lb2 n = Some B2' /\
-    tv_block B1' B2' lc gl.
-Definition tv_blocks__is__correct_prop S1 TD Ps1 F1 lp state1 state2 tr
-  (db:dbBlocks S1 TD Ps1 F1 lp state1 state2 tr) :=
-  forall S2 Ps2 fh1 lb1 fh2 lb2 gl lc n tmn1
-                            l1 ps1 cs1 ps1' l1' als
-                            lc' gl' Mem Mem' als' tmn1' cs1',
-  state1 = (mkState (mkEC (block_intro l1 ps1 cs1 tmn1) lc als) gl Mem) ->
-  state2 = (mkState (mkEC (block_intro l1' ps1' cs1' tmn1') lc' als') gl' Mem') ->
-  tv_system S1 S2 ->
-  tv_products Ps1 Ps2 ->
-  F1 = fdef_intro fh1 lb1 ->
-  tv_fdef (fdef_intro fh1 lb1) (fdef_intro fh2 lb2) gl0 ->
-  tv_blocks lb1 lb2 lc gl ->
-  nth_error lb1 n = Some (block_intro l1 ps1 cs1 tmn1) ->
-  exists l2, exists ps2, exists cs2, exists tmn2, 
-  exists l2', exists ps2', exists cs2', exists tmn2', exists n',
-    nth_error lb2 n = Some (block_intro l2 ps2 cs2 tmn2) /\
-    nth_error lb1 n' = Some (block_intro l1' ps1' cs1' tmn1') /\
-    nth_error lb2 n' = Some (block_intro l2' ps2' cs2' tmn2') /\
-    tv_block (block_intro l1 ps1 cs1 tmn1) (block_intro l2 ps2 cs2 tmn2) lc gl /\
-    tv_block (block_intro l1' ps1' cs1' tmn1') (block_intro l2' ps2' cs2' tmn2') lc gl /\
-    dbBlocks S2 TD Ps2 (fdef_intro fh2 lb2) lp
-      (mkState (mkEC (block_intro l2 ps2 cs2 tmn2) lc als) gl Mem)
-      (mkState (mkEC (block_intro l2' ps2' cs2' tmn2') lc' als') gl' Mem')
-      tr.
-Definition tv_fdef__is__correct_prop fid rt lp S1 TD Ps1 lc gl Mem lc' gl' als' Mem' Rid oResult tr
-  (db:dbFdef fid rt lp S1 TD Ps1 lc gl Mem lc' gl' als' Mem' Rid oResult tr) :=
-  forall Ps2 S2 la lb1,
-  lookupFdefViaIDFromProducts Ps1 fid = Some (fdef_intro (fheader_intro rt fid la) lb1) ->
-  tv_system S1 S2 ->
-  tv_products Ps1 Ps2 ->
-  exists lb2,
-    lookupFdefViaIDFromProducts Ps2 fid = Some (fdef_intro (fheader_intro rt fid la) lb2) /\
-    tv_blocks lb1 lb2 lc gl /\
-    dbFdef fid rt lp S2 TD Ps2 lc gl Mem lc' gl' als' Mem' Rid oResult tr.
-
-Lemma tv_blocks_nth_Some_inv : forall lb1 lb2 lc gl n B1,
-  tv_blocks lb1 lb2 lc gl ->
-  nth_error lb1 n = Some B1 ->
-  exists B2, 
-    nth_error lb2 n = Some B2 /\ tv_block B1 B2 lc gl.
-Admitted. (*nth*)
 
 Lemma cmds2sbs_nil_inv : forall cs,
   cmds2sbs cs = (nil, nil) ->
@@ -639,6 +396,259 @@ Proof.
      simpl. rewrite <- HeqR. rewrite J2. auto.
 Qed.
 
+(* Correctness of the cmds validator *)
+
+Definition tv_cmds (nbs1 nbs2 : list nbranch) (lc gl:GVMap) :=
+se_cmds (mkSstate (env_to_smap gl lc) smem_init sframe_init nil) nbs1 =
+se_cmds (mkSstate (env_to_smap gl lc) smem_init sframe_init nil) nbs2.
+
+Lemma tv_cmds__is__correct : forall TD nbs nbs' lc1 als1 gl1 Mem1 lc2 als2 gl2 Mem2 tr,
+  uniq gl1 ->
+  uniq lc1 ->  
+  wf_nbranchs nbs' ->
+  tv_cmds nbs nbs' lc1 gl1 ->
+  dbCmds TD lc1 als1 gl1 Mem1 (nbranchs2cmds nbs) lc2 als2 gl2 Mem2 tr ->
+  dbCmds TD lc1 als1 gl1 Mem1 (nbranchs2cmds nbs') lc2 als2 gl2 Mem2 tr.
+Proof.
+  intros TD nbs nbs' lc1 als1 gl1 Mem1 lc2 als2 gl2 Mem2 tr Huniqg Huniqc Wf Htv_cmds HdbCmds.
+  unfold tv_cmds in Htv_cmds.
+  assert (Uniqs:=HdbCmds).
+  apply dbCmds_uniq in Uniqs; auto.
+  destruct Uniqs as [Uniqg2 Uniqc2].
+  apply op_cmds__satisfy__se_cmds in HdbCmds; auto.
+  rewrite Htv_cmds in HdbCmds.
+  apply se_cmds__denote__op_cmds; auto.
+Qed.
+
+Definition tv_subblock (sb1 sb2:subblock) (lc gl:GVMap) :=
+match (sb1, sb2) with
+| (mkSB nbs1 call1 iscall1, mkSB nbs2 call2 iscall2) =>
+  let st1 := se_cmds (mkSstate (env_to_smap gl lc) smem_init sframe_init nil) nbs1 in
+  let st2 := se_cmds (mkSstate (env_to_smap gl lc) smem_init sframe_init nil) nbs2 in
+  let cl1 := se_call st1 call1 iscall1 in
+  let cl2 := se_call st2 call2 iscall2 in
+  st1 = st2 /\ call1 = call2
+end.
+
+Fixpoint tv_subblocks (sbs1 sbs2:list subblock) (lc gl:GVMap) :=
+match (sbs1, sbs2) with
+| (nil, nil) => True
+| (sb1::sbs1', sb2::sbs2') => tv_subblock sb1 sb2 lc gl /\ tv_subblocks sbs1' sbs2' lc gl 
+| _ => False
+end.
+
+Fixpoint tv_phinodes (ps1 ps2:list phinode) :=
+match (ps1, ps2) with
+| (nil, nil) => True
+| (p1::ps1', p2::ps2') => p1=p2 /\ tv_phinodes ps1' ps2'
+| _ => False
+end.
+
+Definition tv_block (b1 b2:block) (lc gl:GVMap) :=
+match (b1, b2) with
+| (block_intro l1 ps1 cs1 tmn1, block_intro l2 ps2 cs2 tmn2) =>
+  match (cmds2sbs cs1, cmds2sbs cs2) with
+  | ((sbs1, nbs1), (sbs2, nbs2)) =>
+    l1 = l2 /\ 
+    tv_phinodes ps1 ps2 /\ 
+    tv_subblocks sbs1 sbs2 lc gl /\ 
+    tv_cmds nbs1 nbs2 lc gl /\ 
+    tmn1 = tmn2
+  end
+end.
+
+Fixpoint tv_blocks (bs1 bs2:list block) (lc gl:GVMap) :=
+match (bs1, bs2) with
+| (nil, nil) => True
+| (b1::bs1', b2::bs2') => tv_block b1 b2 lc gl /\ tv_blocks bs1' bs2' lc gl 
+| _ => False
+end.
+
+Variable lc0 gl0 : GVMap.
+
+Definition tv_fdef (f1 f2:fdef) (gl:GVMap) :=
+match (f1, f2) with
+| (fdef_intro fh1 lb1, fdef_intro fh2 lb2) =>
+  fh1 = fh2 /\ tv_blocks lb1 lb2 lc0 gl
+end.
+
+Fixpoint tv_products (Ps1 Ps2:list product):=
+match (Ps1, Ps2) with
+| (nil, nil) => True
+| (product_fdec f1::Ps1', product_fdec f2::Ps2') => 
+  f1 = f2 /\ tv_products Ps1' Ps2'
+| (product_fdef f1::Ps1', product_fdef f2::Ps2') => 
+  tv_fdef f1 f2 gl0 /\ tv_products Ps1' Ps2'
+| (product_gvar gvar1::Ps1', product_gvar gvar2::Ps2') => 
+  gvar1 = gvar2 /\ tv_products Ps1' Ps2'
+| _ => False
+end.
+
+Definition tv_module (m1 m2:module) :=
+match (m1, m2) with
+| (module_intro TD1 Ps1, module_intro TD2 Ps2) =>
+  TD1 = TD2 /\ tv_products Ps1 Ps2
+end.
+
+Fixpoint tv_system (S1 S2:system) :=
+match (S1, S2) with
+| (nil, nil) => True
+| (m1::S1', m2::S2') => tv_module m1 m2 /\ tv_system S1' S2'
+| _ => False
+end.
+
+Inductive wf_subblock : subblock -> Prop :=
+| wf_subblock_intro : forall nbs call0 iscall0, 
+  wf_nbranchs nbs ->
+  wf_subblock (mkSB nbs call0 iscall0).
+
+Inductive wf_subblocks : list subblock -> Prop :=
+| wf_subblocks_nil : wf_subblocks nil
+| wf_subblocks_cons : forall sb sbs,
+  wf_subblock sb ->
+  wf_subblocks sbs ->
+  wf_subblocks (sb::sbs).
+
+Inductive wf_block : block -> Prop :=
+| wf_block_intro : forall l ps cs sbs nbs tmn, 
+  cmds2sbs cs = (sbs,nbs) ->
+  wf_subblocks sbs ->
+  wf_nbranchs nbs ->
+  wf_block (block_intro l ps cs tmn).
+
+Lemma tv_terminator__is__correct : forall TD fh1 lb1 fh2 lb2 B1 B2 lc gl tmn B1' lc' tr,
+  tv_fdef (fdef_intro fh1 lb1) (fdef_intro fh2 lb2) gl0 ->
+  tv_block B1 B2 lc gl ->
+  dbTerminator TD (fdef_intro fh1 lb1) B1 lc gl tmn B1' lc' tr ->
+  exists B2', exists n,
+    tv_block B1' B2' lc gl /\
+    nth_error lb1 n = Some B1' /\
+    nth_error lb2 n = Some B2' /\
+    dbTerminator TD (fdef_intro fh2 lb2) B2 lc gl tmn B2' lc' tr.
+Proof.
+  intros TD fh1 lb1 fh2 lb2 B1 B2 lc gl tmn B1' lc' tr Htv_fdef Htv_block HdbTerminator.
+  inversion HdbTerminator; subst.
+    assert (exists B2', exists n, tv_block (block_intro l' ps' sbs' tmn') B2' lc gl /\ 
+                                  nth_error lb1 n = Some (block_intro l' ps' sbs' tmn') /\
+                                  nth_error lb2 n = Some B2') as J.
+      admit. (*lookup*)
+    destruct J as [B2' [n [J1 [J2 J3]]]].
+    exists B2'. exists n. split; auto. split; auto. split; auto.
+    destruct B2' as [l2' ps2' sbs2' tmn2'].
+    apply dbBranch with (c:=c); auto.
+      admit. (*lookup*)
+      admit. (*switch*)
+    
+    assert (exists B2', exists n, tv_block (block_intro l' ps' sbs' tmn') B2' lc gl /\ 
+                                  nth_error lb1 n = Some (block_intro l' ps' sbs' tmn') /\
+                                  nth_error lb2 n = Some B2') as J.
+      admit. (*lookup*)
+    destruct J as [B2' [n [J1 [J2 J3]]]].
+    exists B2'. exists n. split; auto. split; auto. split; auto.
+    destruct B2' as [l2' ps2' sbs2' tmn2'].
+    apply dbBranch_uncond; auto.
+      admit. (*lookup*)
+      admit. (*switch*)
+Qed.
+
+Lemma tv_blocks_nth_Some_inv : forall lb1 lb2 lc gl n B1,
+  tv_blocks lb1 lb2 lc gl ->
+  nth_error lb1 n = Some B1 ->
+  exists B2, 
+    nth_error lb2 n = Some B2 /\ tv_block B1 B2 lc gl.
+Admitted. (*nth*)
+
+
+Definition tv_dbCall__is__correct_prop S1 TD Ps1 lc gl Mem0 call0 lc' gl' Mem' tr
+  (db:dbCall S1 TD Ps1 lc gl Mem0 call0 lc' gl' Mem' tr) :=
+  forall S2 Ps2,
+  tv_system S1 S2 ->
+  tv_products Ps1 Ps2 ->
+  dbCall S2 TD Ps2 lc gl Mem0 call0 lc' gl' Mem' tr.
+Definition tv_subblock__is__correct_prop S1 TD Ps1 lc als gl Mem cs1 lc' als' gl' Mem' tr
+  (db:dbSubblock S1 TD Ps1 lc als gl Mem cs1 lc' als' gl' Mem' tr) :=
+  forall S2 Ps2 cs2 sb1 sb2,
+  uniq gl ->
+  uniq lc ->
+  cmds2sbs cs1 = (sb1::nil, nil) ->
+  cmds2sbs cs2 = (sb2::nil, nil) ->
+  wf_subblock sb2 ->
+  tv_system S1 S2 ->
+  tv_products Ps1 Ps2 ->
+  tv_subblock sb1 sb2 lc gl ->
+  dbSubblock S2 TD Ps2 lc als gl Mem cs2 lc' als' gl' Mem' tr.
+Definition tv_subblocks__is__correct_prop S1 TD Ps1 lc als gl Mem cs1 lc' als' gl' Mem' tr
+  (db:dbSubblocks S1 TD Ps1 lc als gl Mem cs1 lc' als' gl' Mem' tr) :=
+  forall S2 Ps2 sbs1 sbs2 cs2,
+  uniq gl ->
+  uniq lc ->
+  cmds2sbs cs1 = (sbs1, nil) ->
+  cmds2sbs cs2 = (sbs2, nil) ->
+  wf_subblocks sbs2 ->
+  tv_system S1 S2 ->
+  tv_products Ps1 Ps2 ->
+  tv_subblocks sbs1 sbs2 lc gl ->
+  dbSubblocks S2 TD Ps2 lc als gl Mem cs2 lc' als' gl' Mem' tr.
+Definition tv_block__is__correct_prop S1 TD Ps1 F1 arg state1 state2 tr
+  (db:dbBlock S1 TD Ps1 F1 arg state1 state2 tr) :=
+  forall S2 Ps2 fh1 lb1 fh2 lb2 B1 lc als gl Mem B1' lc' als' gl' Mem' B2,
+  state1 = mkState (mkEC B1 lc als) gl Mem ->
+  state2 = mkState (mkEC B1' lc' als') gl' Mem' ->
+  F1 = fdef_intro fh1 lb1 ->
+  uniq gl ->
+  uniq lc ->
+  wf_block B2 ->
+  tv_system S1 S2 ->
+  tv_products Ps1 Ps2 ->
+  tv_fdef (fdef_intro fh1 lb1) (fdef_intro fh2 lb2) gl0 ->
+  tv_block B1 B2 lc gl ->
+  exists B2', exists n,
+    dbBlock S2 TD Ps2 (fdef_intro fh2 lb2) arg 
+      (mkState (mkEC B2 lc als) gl Mem) 
+      (mkState (mkEC B2' lc' als') gl' Mem')
+      tr /\
+    nth_error lb1 n = Some B1' /\
+    nth_error lb2 n = Some B2' /\
+    tv_block B1' B2' lc gl.
+Definition tv_blocks__is__correct_prop S1 TD Ps1 F1 lp state1 state2 tr
+  (db:dbBlocks S1 TD Ps1 F1 lp state1 state2 tr) :=
+  forall S2 Ps2 fh1 lb1 fh2 lb2 gl lc n tmn1
+                            l1 ps1 cs1 ps1' l1' als
+                            lc' gl' Mem Mem' als' tmn1' cs1',
+  state1 = (mkState (mkEC (block_intro l1 ps1 cs1 tmn1) lc als) gl Mem) ->
+  state2 = (mkState (mkEC (block_intro l1' ps1' cs1' tmn1') lc' als') gl' Mem') ->
+  tv_system S1 S2 ->
+  tv_products Ps1 Ps2 ->
+  F1 = fdef_intro fh1 lb1 ->
+  tv_fdef (fdef_intro fh1 lb1) (fdef_intro fh2 lb2) gl0 ->
+  tv_blocks lb1 lb2 lc gl ->
+  nth_error lb1 n = Some (block_intro l1 ps1 cs1 tmn1) ->
+  exists l2, exists ps2, exists cs2, exists tmn2, 
+  exists l2', exists ps2', exists cs2', exists tmn2', exists n',
+    nth_error lb2 n = Some (block_intro l2 ps2 cs2 tmn2) /\
+    nth_error lb1 n' = Some (block_intro l1' ps1' cs1' tmn1') /\
+    nth_error lb2 n' = Some (block_intro l2' ps2' cs2' tmn2') /\
+    tv_block (block_intro l1 ps1 cs1 tmn1) (block_intro l2 ps2 cs2 tmn2) lc gl /\
+    tv_block (block_intro l1' ps1' cs1' tmn1') (block_intro l2' ps2' cs2' tmn2') lc gl /\
+    dbBlocks S2 TD Ps2 (fdef_intro fh2 lb2) lp
+      (mkState (mkEC (block_intro l2 ps2 cs2 tmn2) lc als) gl Mem)
+      (mkState (mkEC (block_intro l2' ps2' cs2' tmn2') lc' als') gl' Mem')
+      tr.
+Definition tv_fdef__is__correct_prop fid rt lp S1 TD Ps1 lc gl Mem lc' gl' als' Mem' B1' Rid oResult tr
+  (db:dbFdef fid rt lp S1 TD Ps1 lc gl Mem lc' gl' als' Mem' B1' Rid oResult tr) :=
+  forall Ps2 S2 la lb1,
+  lookupFdefViaIDFromProducts Ps1 fid = Some (fdef_intro (fheader_intro rt fid la) lb1) ->
+  tv_system S1 S2 ->
+  tv_products Ps1 Ps2 ->
+  exists lb2, exists B2', exists n,
+    nth_error lb1 n = Some B1' /\
+    nth_error lb2 n = Some B2' /\
+    tv_block B1' B2' lc gl /\
+    lookupFdefViaIDFromProducts Ps2 fid = Some (fdef_intro (fheader_intro rt fid la) lb2) /\
+    tv_blocks lb1 lb2 lc gl /\
+    dbFdef fid rt lp S2 TD Ps2 lc gl Mem lc' gl' als' Mem' B2' Rid oResult tr.
+
+
 Lemma tv__is__correct :
   (forall S1 TD Ps1 lc gl Mem0 call0 lc' gl' Mem' tr db, 
      tv_dbCall__is__correct_prop S1 TD Ps1 lc gl Mem0 call0 lc' gl' Mem' tr db) /\
@@ -650,8 +660,8 @@ Lemma tv__is__correct :
      tv_block__is__correct_prop S1 TD Ps1 F1 arg state1 state2 tr db) /\
   (forall S1 TD Ps1 F1 lp state1 state2 tr db,
      tv_blocks__is__correct_prop S1 TD Ps1 F1 lp state1 state2 tr db) /\
-  (forall fid rt lp S1 TD Ps1 lc gl Mem lc' gl' als' Mem' Rid oResult tr db,
-     tv_fdef__is__correct_prop fid rt lp S1 TD Ps1 lc gl Mem lc' gl' als' Mem' Rid oResult tr db).
+  (forall fid rt lp S1 TD Ps1 lc gl Mem lc' gl' als' Mem' B' Rid oResult tr db,
+     tv_fdef__is__correct_prop fid rt lp S1 TD Ps1 lc gl Mem lc' gl' als' Mem' B' Rid oResult tr db).
 Proof.
 (db_mutind_cases
   apply db_mutind with
@@ -669,12 +679,12 @@ Case "dbCall_intro".
   inversion d; subst.
     apply H with (S2:=S2)(Ps2:=Ps2) in H2; auto.
     clear H.
-    destruct H2 as [lb2 [J1 [J2 J3]]].
+    destruct H2 as [lb2 [B2' [n [J1 [J2 [J3 [J4 [J5 J6]]]]]]]].
     eauto.
 
     apply H with (S2:=S2)(Ps2:=Ps2) in H2; auto.
     clear H.
-    destruct H2 as [lb2 [J1 [J2 J3]]].
+    destruct H2 as [lb2 [B2' [n [J1 [J2 [J3 [J4 [J5 J6]]]]]]]].
     eauto.
 
 Case "dbSubblock_intro".
@@ -835,7 +845,6 @@ Case "dbFdef_func".
       clear - H1 H3.
       admit. (*lookup*)
     destruct J as [lb2 [H4 H5]].
-    exists lb2. split; auto. split; auto.
     assert (tv_blocks lb lb2 (initLocals la (params2GVs TD lp lc gl)) gl) as Htv_blocks.
       clear - H5.
       admit. (*tv inclusion*)      
@@ -846,8 +855,14 @@ Case "dbFdef_func".
       clear H.
       destruct Htv_blocks as [l3 [ps3 [cs3 [tmn2 [l2' [ps2' [cs2' [tmn2' [n' [J1 [J2 [J3 [J4 [J5 J6]]]]]]]]]]]]]].
 
-      unfold tv_block in J5.
+      exists lb2. exists (block_intro l2' ps2' cs2' tmn2'). exists n'.
+      split; auto. split; auto.
+      split.
+        clear - J5.
+        admit. (*tv inclusion*)      
+      split; auto. split; auto.
 
+      unfold tv_block in J5.
       remember (cmds2sbs (cs21++cs22)) as R1.
       remember (cmds2sbs cs2') as R2.
       destruct R1 as [sbs1 nbs1].
@@ -893,7 +908,7 @@ Case "dbFdef_func".
         apply tv_cmds__is__correct with (nbs':=nbs2) in d1; auto.
           apply dbFdef_func with (l1:=l3)(ps1:=ps3)(cs1:=cs3)(tmn1:=tmn2)(la:=la)(lb:=lb2)
             (lc1:=lc1)(gl1:=gl1)(Mem1:=Mem1)(als1:=als1)(l2:=l2')(ps2:=ps2')(cs21:=cs41)(cs22:=nbranchs2cmds nbs2)
-            (lc3:=lc3)(als3:=als3)(gl3:=gl3)(Mem3:=Mem3); eauto.
+            (lc3:=lc3)(als3:=als3)(gl3:=gl3)(Mem3:=Mem3)(lc2:=lc2)(als2:=als2)(gl2:=gl2)(Mem2:=Mem2); eauto.
           admit. (*Wf*) 
         admit. (*Wf*) 
 
@@ -909,7 +924,6 @@ Case "dbFdef_proc".
       clear - H1 H3.
       admit.  (*lookup*)
     destruct J as [lb2 [H4 H5]].
-    exists lb2. split; auto. split; auto.
     assert (tv_blocks lb lb2 (initLocals la (params2GVs TD lp lc gl)) gl) as Htv_blocks.
       clear - H5.
       admit. (*tv inclusion*)      
@@ -920,8 +934,14 @@ Case "dbFdef_proc".
       clear H.
       destruct Htv_blocks as [l3 [ps3 [cs3 [tmn2 [l2' [ps2' [cs2' [tmn2' [n' [J1 [J2 [J3 [J4 [J5 J6]]]]]]]]]]]]]].
 
-      unfold tv_block in J5.
+      exists lb2. exists (block_intro l2' ps2' cs2' tmn2'). exists n'.
+      split; auto. split; auto.
+      split.
+        clear - J5.
+        admit. (*tv inclusion*)      
+      split; auto. split; auto.
 
+      unfold tv_block in J5.
       remember (cmds2sbs (cs21++cs22)) as R1.
       remember (cmds2sbs cs2') as R2.
       destruct R1 as [sbs1 nbs1].
@@ -967,7 +987,7 @@ Case "dbFdef_proc".
         apply tv_cmds__is__correct with (nbs':=nbs2) in d1; auto.
           apply dbFdef_proc with (l1:=l3)(ps1:=ps3)(cs1:=cs3)(tmn1:=tmn2)(la:=la)(lb:=lb2)
             (lc1:=lc1)(gl1:=gl1)(Mem1:=Mem1)(als1:=als1)(l2:=l2')(ps2:=ps2')(cs21:=cs41)(cs22:=nbranchs2cmds nbs2)
-            (lc3:=lc3)(als3:=als3)(gl3:=gl3)(Mem3:=Mem3); eauto.
+            (lc3:=lc3)(als3:=als3)(gl3:=gl3)(Mem3:=Mem3)(lc2:=lc2)(als2:=als2)(gl2:=gl2)(Mem2:=Mem2); eauto.
           admit. (*Wf*) 
         admit. (*Wf*) 
 
@@ -1078,21 +1098,47 @@ Proof.
   eapply J with (state1:=(mkState (mkEC (block_intro l1 ps1 sbs1 tmn1) lc als) gl Mem0))(state2:=(mkState (mkEC (block_intro l1' ps1' sbs1' tmn1') lc' als') gl' Mem'))(F1:=(fdef_intro fh1 lb1)); eauto.
 Qed.
 
-Lemma tv_fdef__is__correct : forall fid rt lp S1 TD Ps1 lc gl Mem lc' gl' als' Mem' Rid oResult tr
+Lemma _tv_fdef__is__correct : forall fid rt lp S1 TD Ps1 lc gl Mem lc' gl' als' Mem' B1' Rid oResult tr
   Ps2 S2 la lb1,
-  dbFdef fid rt lp S1 TD Ps1 lc gl Mem lc' gl' als' Mem' Rid oResult tr ->
+  dbFdef fid rt lp S1 TD Ps1 lc gl Mem lc' gl' als' Mem' B1' Rid oResult tr ->
   lookupFdefViaIDFromProducts Ps1 fid = Some (fdef_intro (fheader_intro rt fid la) lb1) ->
   tv_system S1 S2 ->
   tv_products Ps1 Ps2 ->
-  exists lb2,
+  exists lb2, exists B2', exists n,
+    nth_error lb1 n = Some B1' /\
+    nth_error lb2 n = Some B2' /\
+    tv_block B1' B2' lc gl /\
     lookupFdefViaIDFromProducts Ps2 fid = Some (fdef_intro (fheader_intro rt fid la) lb2) /\
     tv_blocks lb1 lb2 lc gl /\
-    dbFdef fid rt lp S2 TD Ps2 lc gl Mem lc' gl' als' Mem' Rid oResult tr.
+    dbFdef fid rt lp S2 TD Ps2 lc gl Mem lc' gl' als' Mem' B2' Rid oResult tr.
 Proof.
   intros.
   destruct tv__is__correct as [_ [_ [_ [_ [_ J]]]]].
   unfold tv_fdef__is__correct_prop in J.
   eapply J; eauto.
+Qed.
+
+Lemma tv_fdef__is__correct : forall ECs fid rt lp S1 TD Ps1 lc gl Mem lc' gl' als' Mem' B1' Rid oResult tr
+  Ps2 S2 la lb1,
+  LLVMopsem.dbFdef fid rt lp S1 TD Ps1 ECs lc gl Mem lc' gl' als' Mem' B1' Rid oResult tr ->
+  lookupFdefViaIDFromProducts Ps1 fid = Some (fdef_intro (fheader_intro rt fid la) lb1) ->
+  tv_system S1 S2 ->
+  tv_products Ps1 Ps2 ->
+  exists lb2, exists B2', exists n,
+    nth_error lb1 n = Some B1' /\
+    nth_error lb2 n = Some B2' /\
+    tv_block B1' B2' lc gl /\
+    lookupFdefViaIDFromProducts Ps2 fid = Some (fdef_intro (fheader_intro rt fid la) lb2) /\
+    tv_blocks lb1 lb2 lc gl /\
+    LLVMopsem.dbFdef fid rt lp S2 TD Ps2 ECs lc gl Mem lc' gl' als' Mem' B2' Rid oResult tr.
+Proof.
+  intros.
+  apply llvmop_dbFdef__seop_dbFdef in H.
+  apply _tv_fdef__is__correct with (Ps2:=Ps2)(S2:=S2)(la:=la)(lb1:=lb1) in H; auto.
+  destruct H as [lb2 [B2' [n [J1 [J2 [J3 [J4 [J5 J6]]]]]]]].
+  exists lb2. exists B2'. exists n.
+  repeat (split; auto).
+    apply seop_dbFdef__llvmop_dbFdef; auto.
 Qed.
 
 Extraction "symexe" tv_blocks.
