src/TV/seop_llvmop.v
@@ -1,0 +1,1048 @@
+Add LoadPath "../ssa/ott".
+Add LoadPath "../ssa/monads".
+Add LoadPath "../ssa".
+Add LoadPath "../../../theory/metatheory".
+Require Import ssa.
+Require Import List.
+Require Export targetdata.
+Require Import monad.
+Require Import Arith.
+Require Import Metatheory.
+Require Import ssa_mem.
+Require Import genericvalues.
+Require Import ssa_dynamic.
+Require Import opsem_conv.
+Require Import trace.
+Require Import symexe_def.
+
+Export LLVMsyntax.
+Export LLVMlib.
+
+Tactic Notation "se_db_mutind_cases" tactic(first) tactic(c) :=
+  first;
+  [ c "dbCall_intro" | 
+    c "dbSubblock_intro" | c "dbSubblocks_nil" | c "dbSubblocks_cons" | 
+    c "dbBlock_intro" | c "dbBlocks_nil" | c "dbBlocks_cons" | 
+    c "dbFdef_func" | c "dbFdef_proc" ].
+
+Tactic Notation "se_dbCmd_cases" tactic(first) tactic(c) :=
+  first;
+  [ c "dbBop" | c "dbExtractValue" | c "dbInsertValue" |
+    c "dbMalloc" | c "dbFree" |
+    c "dbAlloca" | c "dbLoad" | c "dbStore" | c "dbGEP" |
+    c "dbExt" | c "dbCast" | c "dbIcmp" |  c "dbSelect" ].
+
+Tactic Notation "se_dbTerminator_cases" tactic(first) tactic(c) :=
+  first;
+  [ c "dbBranch" | c "dbBranch_uncond" ].
+
+Tactic Notation "se_dbCmds_cases" tactic(first) tactic(c) :=
+  first;
+  [ c "dbCmds_nil" | c "dbCmds_cons" ].
+
+(****************************************************)
+(* seop -> llvmop *)
+
+Lemma seop_dbCmd__llvmop_dbInsn : forall TD lc als gl Mem c lc' gl' als' Mem' tr S Ps F B ECs arg tmn cs,
+  SimpleSE.dbCmd TD lc als gl Mem c lc' als' gl' Mem' tr ->
+  LLVMopsem.dbInsn 
+    (mkState S TD Ps ((mkEC F B (c::cs) tmn lc arg als)::ECs) gl Mem)
+    (mkState S TD Ps ((mkEC F B cs tmn lc' arg als')::ECs) gl' Mem')
+    tr.
+Proof.
+  intros TD lc als gl Mem0 c lc' gl' als' Mem' tr S Ps F B ECs arg0 tmn cs H.
+  (se_dbCmd_cases (destruct H) Case); eauto.
+Qed.
+  
+Lemma seop_dbCmds__llvmop_dbop : forall TD lc als gl Mem cs cs' lc' gl' als' Mem' tr S Ps F B ECs arg tmn,
+  SimpleSE.dbCmds TD lc als gl Mem cs lc' als' gl' Mem' tr ->
+  LLVMopsem.dbop 
+    (mkState S TD Ps ((mkEC F B (cs++cs') tmn lc arg als)::ECs) gl Mem)
+    (mkState S TD Ps ((mkEC F B cs' tmn lc' arg als')::ECs) gl' Mem')
+    tr.
+Proof.
+  intros TD lc als gl Mem0 cs cs' lc' gl' als' Mem' tr S Ps F B ECs arg0 tmn H.
+  generalize dependent S.
+  generalize dependent Ps.
+  generalize dependent F.
+  generalize dependent B.
+  generalize dependent ECs.
+  generalize dependent arg0.
+  generalize dependent tmn.
+  generalize dependent cs'.
+  (se_dbCmds_cases (induction H) Case);intros; auto.
+    simpl_env.
+    apply seop_dbCmd__llvmop_dbInsn with (S:=S)(Ps:=Ps)(F:=F)(B:=B)(ECs:=ECs)(arg:=arg0)(tmn:=tmn)(cs:=cs++cs') in H; auto.
+    eapply dbop_cons; eauto.
+      apply IHdbCmds.
+Qed.
+
+Lemma seop_dbTerminator__llvmop_dbInsn : forall TD lc als gl Mem lc' tr S Ps F B ECs arg tmn l' ps' cs' tmn',
+  SimpleSE.dbTerminator TD F B lc gl tmn (block_intro l' ps' cs' tmn') lc' tr ->
+  LLVMopsem.dbInsn 
+    (mkState S TD Ps ((mkEC F B nil tmn lc arg als)::ECs) gl Mem)
+    (mkState S TD Ps ((mkEC F (block_intro l' ps' cs' tmn') cs' tmn' lc' arg als)::ECs) gl Mem)
+    tr.
+Proof.
+  intros TD lc als gl Mem0 lc' tr S Ps F B ECs arg0 tmn l' ps' cs' tmn' H.
+  inversion H; subst.
+    eapply dbBranch; eauto.
+      rewrite H13.
+      admit. (*lookup*)
+    eapply dbBranch_uncond; eauto.    
+      rewrite H12.
+      admit. (*lookup*)
+Qed.
+
+Definition seop_dbCall__llvmop_dbCall_prop S TD Ps lc gl Mem0 call0 lc' gl' Mem' tr
+  (db:SimpleSE.dbCall S TD Ps lc gl Mem0 call0 lc' gl' Mem' tr) :=
+  forall F B ECs arg tmn cs als,
+  LLVMopsem.dbInsn 
+    (mkState S TD Ps ((mkEC F B (call0::cs) tmn lc arg als)::ECs) gl Mem0)
+    (mkState S TD Ps ((mkEC F B cs tmn lc' arg als)::ECs) gl' Mem')
+    tr.
+Definition seop_dbSubblock__llvmop_dbop_prop S TD Ps lc als gl Mem cs lc' als' gl' Mem' tr
+  (db:SimpleSE.dbSubblock S TD Ps lc als gl Mem cs lc' als' gl' Mem' tr) :=
+  forall F B ECs arg tmn cs',
+  LLVMopsem.dbop 
+    (mkState S TD Ps ((mkEC F B (cs++cs') tmn lc arg als)::ECs) gl Mem)
+    (mkState S TD Ps ((mkEC F B cs' tmn lc' arg als')::ECs) gl' Mem')
+    tr.
+Definition seop_dbSubblocks__llvmop_dbop_prop S TD Ps lc als gl Mem cs lc' als' gl' Mem' tr
+  (db:SimpleSE.dbSubblocks S TD Ps lc als gl Mem cs lc' als' gl' Mem' tr) :=
+  forall F B ECs arg tmn cs',
+  LLVMopsem.dbop 
+    (mkState S TD Ps ((mkEC F B (cs++cs') tmn lc arg als)::ECs) gl Mem)
+    (mkState S TD Ps ((mkEC F B cs' tmn lc' arg als')::ECs) gl' Mem')
+    tr.
+Definition seop_dbBlock__llvmop_dbop_prop S TD Ps F arg state state' tr
+  (db:SimpleSE.dbBlock S TD Ps F arg state state' tr) :=
+  forall l ps cs tmn lc als gl Mem l' ps' cs' tmn' lc' als' gl' Mem' ECs,
+  state = SimpleSE.mkState (SimpleSE.mkEC (block_intro l ps cs tmn) lc als) gl Mem ->
+  state' = SimpleSE.mkState (SimpleSE.mkEC (block_intro l' ps' cs' tmn') lc' als') gl' Mem' ->
+  LLVMopsem.dbop 
+    (mkState S TD Ps ((mkEC F (block_intro l ps cs tmn) cs tmn lc arg als)::ECs) gl Mem)
+    (mkState S TD Ps ((mkEC F (block_intro l' ps' cs' tmn') cs' tmn' lc' arg als')::ECs) gl' Mem')
+    tr.
+Definition seop_dbBlocks__llvmop_dbop_prop S TD Ps F arg state state' tr
+  (db:SimpleSE.dbBlocks S TD Ps F arg state state' tr) :=
+  forall l ps cs tmn lc als gl Mem l' ps' cs' tmn' lc' als' gl' Mem' ECs,
+  state = SimpleSE.mkState (SimpleSE.mkEC (block_intro l ps cs tmn) lc als) gl Mem ->
+  state' = SimpleSE.mkState (SimpleSE.mkEC (block_intro l' ps' cs' tmn') lc' als') gl' Mem' ->
+  LLVMopsem.dbop 
+    (mkState S TD Ps ((mkEC F (block_intro l ps cs tmn) cs tmn lc arg als)::ECs) gl Mem)
+    (mkState S TD Ps ((mkEC F (block_intro l' ps' cs' tmn') cs' tmn' lc' arg als')::ECs) gl' Mem')
+    tr.
+Definition seop_dbFdef__llvmop_dbFdef_prop fid rt lp S TD Ps lc gl Mem lc' gl' als' Mem' B' Rid oResult tr
+  (db:SimpleSE.dbFdef fid rt lp S TD Ps lc gl Mem lc' gl' als' Mem' B' Rid oResult tr) :=
+  forall ECs,
+  LLVMopsem.dbFdef fid rt lp S TD Ps ECs lc gl Mem lc' gl' als' Mem' B' Rid oResult tr.
+
+Lemma dbop_trans : forall state1 state2 state3 tr1 tr2,
+  dbop state1 state2 tr1 ->
+  dbop state2 state3 tr2 ->
+  dbop state1 state3 (trace_app tr1 tr2).
+Proof.
+  intros state1 state2 state3 tr1 tr2 H.
+  generalize dependent state3.
+  generalize dependent tr2.
+  induction H; intros; auto.
+    rewrite <- trace_app_commute. eauto.
+Qed.
+
+Lemma dbInsn__dbop : forall state1 state2 tr,
+  dbInsn state1 state2 tr ->
+  dbop state1 state2 tr.
+Proof.
+  intros.
+  rewrite <- trace_app_nil__eq__trace.
+  eapply dbop_cons; eauto.
+Qed.
+
+Lemma seop__llvmop :
+  (forall S1 TD Ps1 lc gl Mem0 call0 lc' gl' Mem' tr db, 
+     seop_dbCall__llvmop_dbCall_prop S1 TD Ps1 lc gl Mem0 call0 lc' gl' Mem' tr db) /\
+  (forall S1 TD Ps1 lc als gl Mem sb1 lc' als' gl' Mem' tr db,
+     seop_dbSubblock__llvmop_dbop_prop S1 TD Ps1 lc als gl Mem sb1 lc' als' gl' Mem' tr db) /\
+  (forall S1 TD Ps1 lc als gl Mem sbs1 lc' als' gl' Mem' tr db,
+     seop_dbSubblocks__llvmop_dbop_prop S1 TD Ps1 lc als gl Mem sbs1 lc' als' gl' Mem' tr db) /\
+  (forall S1 TD Ps1 F1 arg state1 state2 tr db,
+     seop_dbBlock__llvmop_dbop_prop S1 TD Ps1 F1 arg state1 state2 tr db) /\
+  (forall S1 TD Ps1 F1 lp state1 state2 tr db,
+     seop_dbBlocks__llvmop_dbop_prop S1 TD Ps1 F1 lp state1 state2 tr db) /\
+  (forall fid rt lp S1 TD Ps1 lc gl Mem lc' gl' als' Mem' B' Rid oResult tr db,
+     seop_dbFdef__llvmop_dbFdef_prop fid rt lp S1 TD Ps1 lc gl Mem lc' gl' als' Mem' B' Rid oResult tr db).
+Proof.
+(se_db_mutind_cases
+  apply SimpleSE.db_mutind with
+    (P  := seop_dbCall__llvmop_dbCall_prop)
+    (P0 := seop_dbSubblock__llvmop_dbop_prop)
+    (P1 := seop_dbSubblocks__llvmop_dbop_prop)
+    (P2 := seop_dbBlock__llvmop_dbop_prop)
+    (P3 := seop_dbBlocks__llvmop_dbop_prop)
+    (P4 := seop_dbFdef__llvmop_dbFdef_prop) Case);
+  unfold seop_dbCall__llvmop_dbCall_prop, 
+         seop_dbFdef__llvmop_dbFdef_prop, seop_dbSubblock__llvmop_dbop_prop,
+         seop_dbSubblocks__llvmop_dbop_prop, seop_dbBlock__llvmop_dbop_prop,
+         seop_dbBlocks__llvmop_dbop_prop; intros; subst; eauto.
+Case "dbSubblock_intro".
+  apply seop_dbCmds__llvmop_dbop with (Ps:=Ps)(F:=F)(B:=B)(ECs:=ECs)(arg:=arg0)(tmn:=tmn)(S:=S)(cs':=call0::cs') in d.
+  eapply dbop_trans; simpl_env ; eauto.
+    apply dbInsn__dbop; auto. 
+      apply H.
+Case "dbSubblocks_cons".
+  rewrite app_ass.
+  apply dbop_trans with (state2:=mkState S TD Ps (mkEC F B (cs'++cs'0) tmn lc2 arg0 als2::ECs) gl2 Mem2); eauto.
+Case "dbBlock_intro".
+  inversion H0; subst. clear H0.
+  inversion H1; subst. clear H1.
+  rewrite <- trace_app_commute.
+  apply dbop_trans with (state2:=mkState S TD Ps (mkEC F (block_intro l1 ps0 (cs++cs') tmn0) cs' tmn0 lc2 arg0 als2::ECs) gl2 Mem2); eauto.
+    apply seop_dbCmds__llvmop_dbop with (Ps:=Ps)(F:=F)(B:=block_intro l1 ps0 (cs++cs') tmn0)(ECs:=ECs)(arg:=arg0)(S:=S)(cs':=nil)(tmn:=tmn0) in d0.
+    apply seop_dbTerminator__llvmop_dbInsn with (Ps:=Ps)(F:=F)(ECs:=ECs)(arg:=arg0)(S:=S)(als:=als')(Mem:=Mem') in d1.
+    simpl_env in d0.
+    apply dbop_trans with (state2:=mkState S TD Ps (mkEC F (block_intro l1 ps0 (cs++cs') tmn0) nil tmn0 lc3 arg0 als'::ECs) gl' Mem'); auto.
+      apply dbInsn__dbop; auto. 
+Case "dbBlocks_nil".
+  inversion H0; subst. clear H0.
+  auto.
+Case "dbBlocks_cons".
+  inversion d; subst.
+  destruct B'.
+  apply dbop_trans with (state2:=mkState S TD Ps (mkEC F (block_intro l1 l2 l3 t) l3 t lc4 arg0 als3::ECs) gl3 Mem3); eauto.
+Case "dbFdef_func".
+  apply dbFdef_func with (l':=l1)(ps':=ps1)(cs':=cs1)(tmn':=tmn1)(la:=la)(lb:=lb); auto.
+    rewrite <- e. 
+    admit. (*lookup*)
+
+    rewrite <- trace_app_commute.
+    apply seop_dbCmds__llvmop_dbop with (Ps:=Ps)(F:=fdef_intro (fheader_intro rt fid la) lb)(B:=block_intro l2 ps2 (cs21++cs22) (insn_return rid rt Result))(ECs:=ECs)(arg:=(params2GVs TD lp lc gl))(S:=S)(cs':=nil)(tmn:=insn_return rid rt Result) in d1.
+    simpl_env in d1. 
+    apply dbop_trans with (state2:=mkState S TD Ps (mkEC (fdef_intro (fheader_intro rt fid la) lb) (block_intro l2 ps2 (cs21++cs22) (insn_return rid rt Result)) (cs21++cs22) (insn_return rid rt Result) lc1 (params2GVs TD lp lc gl) als1::ECs) gl1 Mem1); auto.
+    apply dbop_trans with (state2:=mkState S TD Ps (mkEC (fdef_intro (fheader_intro rt fid la) lb) (block_intro l2 ps2 (cs21++cs22) (insn_return rid rt Result)) cs22 (insn_return rid rt Result) lc2 (params2GVs TD lp lc gl) als2::ECs) gl2 Mem2); auto.
+Case "dbFdef_proc".
+  apply dbFdef_proc with (l':=l1)(ps':=ps1)(cs':=cs1)(tmn':=tmn1)(la:=la)(lb:=lb); auto.
+    rewrite <- e. 
+    admit. (*lookup*)
+
+    rewrite <- trace_app_commute.
+    apply seop_dbCmds__llvmop_dbop with (Ps:=Ps)(F:=fdef_intro (fheader_intro rt fid la) lb)(B:=block_intro l2 ps2 (cs21++cs22) (insn_return_void rid))(ECs:=ECs)(arg:=(params2GVs TD lp lc gl))(S:=S)(cs':=nil)(tmn:=insn_return_void rid) in d1.
+    simpl_env in d1. 
+    apply dbop_trans with (state2:=mkState S TD Ps (mkEC (fdef_intro (fheader_intro rt fid la) lb) (block_intro l2 ps2 (cs21++cs22) (insn_return_void rid)) (cs21++cs22) (insn_return_void rid) lc1 (params2GVs TD lp lc gl) als1::ECs) gl1 Mem1); auto.
+    apply dbop_trans with (state2:=mkState S TD Ps (mkEC (fdef_intro (fheader_intro rt fid la) lb) (block_intro l2 ps2 (cs21++cs22) (insn_return_void rid)) cs22 (insn_return_void rid) lc2 (params2GVs TD lp lc gl) als2::ECs) gl2 Mem2); auto.
+Qed.
+
+Lemma seop_dbCall__llvmop_dbCall : forall S TD Ps lc gl Mem0 call0 lc' gl' Mem' tr F B ECs arg tmn cs als,
+  SimpleSE.dbCall S TD Ps lc gl Mem0 call0 lc' gl' Mem' tr ->
+  LLVMopsem.dbInsn 
+    (mkState S TD Ps ((mkEC F B (call0::cs) tmn lc arg als)::ECs) gl Mem0)
+    (mkState S TD Ps ((mkEC F B cs tmn lc' arg als)::ECs) gl' Mem')
+    tr.
+Proof.
+  intros.
+  destruct seop__llvmop as [J _]. 
+  apply J; auto.
+Qed.
+
+Lemma seop_dbSubblock__llvmop_dbop : forall S TD Ps lc als gl Mem cs lc' als' gl' Mem' tr F B ECs arg tmn cs',
+  SimpleSE.dbSubblock S TD Ps lc als gl Mem cs lc' als' gl' Mem' tr ->
+  LLVMopsem.dbop 
+    (mkState S TD Ps ((mkEC F B (cs++cs') tmn lc arg als)::ECs) gl Mem)
+    (mkState S TD Ps ((mkEC F B cs' tmn lc' arg als')::ECs) gl' Mem')
+    tr.
+Proof.
+  intros.
+  destruct seop__llvmop as [_ [J _]]. 
+  apply J; auto.
+Qed.
+
+Lemma seop_dbSubblocks__llvmop_dbop : forall S TD Ps lc als gl Mem cs lc' als' gl' Mem' tr F B ECs arg tmn cs',
+  SimpleSE.dbSubblocks S TD Ps lc als gl Mem cs lc' als' gl' Mem' tr ->
+  LLVMopsem.dbop 
+    (mkState S TD Ps ((mkEC F B (cs++cs') tmn lc arg als)::ECs) gl Mem)
+    (mkState S TD Ps ((mkEC F B cs' tmn lc' arg als')::ECs) gl' Mem')
+    tr.
+Proof.
+  intros.
+  destruct seop__llvmop as [_ [_ [J _]]]. 
+  apply J; auto.
+Qed.
+
+Lemma seop_dbBlock__llvmop_dbop :  forall S TD Ps F arg tr l ps cs tmn lc als gl Mem l' ps' cs' tmn' lc' als' gl' Mem' ECs,
+  SimpleSE.dbBlock S TD Ps F arg 
+    (SimpleSE.mkState (SimpleSE.mkEC (block_intro l ps cs tmn) lc als) gl Mem) 
+    (SimpleSE.mkState (SimpleSE.mkEC (block_intro l' ps' cs' tmn') lc' als') gl' Mem')
+    tr ->
+  LLVMopsem.dbop 
+    (mkState S TD Ps ((mkEC F (block_intro l ps cs tmn) cs tmn lc arg als)::ECs) gl Mem)
+    (mkState S TD Ps ((mkEC F (block_intro l' ps' cs' tmn') cs' tmn' lc' arg als')::ECs) gl' Mem')
+    tr.
+Proof.
+  intros.
+  destruct seop__llvmop as [_ [_ [_ [J _]]]]. 
+  unfold seop_dbBlock__llvmop_dbop_prop in J.
+  eapply J; eauto.
+Qed.
+
+Lemma seop_dbBlocks__llvmop_dbop : forall S TD Ps F arg tr l ps cs tmn lc als gl Mem l' ps' cs' tmn' lc' als' gl' Mem' ECs,
+  SimpleSE.dbBlocks S TD Ps F arg 
+    (SimpleSE.mkState (SimpleSE.mkEC (block_intro l ps cs tmn) lc als) gl Mem) 
+    (SimpleSE.mkState (SimpleSE.mkEC (block_intro l' ps' cs' tmn') lc' als') gl' Mem')
+    tr ->  
+  LLVMopsem.dbop 
+    (mkState S TD Ps ((mkEC F (block_intro l ps cs tmn) cs tmn lc arg als)::ECs) gl Mem)
+    (mkState S TD Ps ((mkEC F (block_intro l' ps' cs' tmn') cs' tmn' lc' arg als')::ECs) gl' Mem')
+    tr.
+Proof.
+  intros.
+  destruct seop__llvmop as [_ [_ [_ [_ [J _]]]]]. 
+  unfold seop_dbBlocks__llvmop_dbop_prop in J.
+  eapply J; eauto.
+Qed.
+
+Lemma seop_dbFdef__llvmop_dbFdef : forall fid rt lp S TD Ps lc gl Mem lc' gl' als' Mem' B' Rid oResult tr ECs,
+  SimpleSE.dbFdef fid rt lp S TD Ps lc gl Mem lc' gl' als' Mem' B' Rid oResult tr ->
+  LLVMopsem.dbFdef fid rt lp S TD Ps ECs lc gl Mem lc' gl' als' Mem' B' Rid oResult tr.
+Proof.
+  intros.
+  destruct seop__llvmop as [_ [_ [_ [_ [_ J]]]]]. 
+  eapply J; eauto.
+Qed.
+
+(****************************************************)
+(* llvmop -> seop *)
+
+Lemma dbBlock__dbBlocks : forall S TD Ps F arg state state' tr,
+  SimpleSE.dbBlock S TD Ps F arg state state' tr -> 
+  SimpleSE.dbBlocks S TD Ps F arg state state' tr.
+Proof.
+  intros S TD Ps F arg0 state state' tr H.
+  rewrite <- trace_app_nil__eq__trace.
+  eapply SimpleSE.dbBlocks_cons; eauto.
+Qed.
+
+Lemma dbTerminator__dbBlock : forall TD F lc gl tmn l ps B' lc' tr als Ps S arg Mem,
+  SimpleSE.dbTerminator TD F (block_intro l ps nil tmn) lc gl tmn B' lc' tr ->
+  SimpleSE.dbBlock S TD Ps F arg 
+    (SimpleSE.mkState (SimpleSE.mkEC (block_intro l ps nil tmn) lc als) gl Mem)
+    (SimpleSE.mkState (SimpleSE.mkEC B' lc' als) gl Mem)
+    tr.
+Proof.
+  intros TD F lc gl tmn l0 ps B' lc' tr als Ps S arg0 Mem0 H.
+  rewrite <- nil_app_trace__eq__trace.
+  rewrite <- nil_app_trace__eq__trace with (tr:=trace_nil).
+  assert (@nil cmd=nil++nil) as EQ. auto.
+  rewrite EQ.
+  apply SimpleSE.dbBlock_intro with (lc2:=lc)(als2:=als)(gl2:=gl)(Mem2:=Mem0)(lc3:=lc); auto.
+Qed.
+
+Lemma dbCmd_dbSubblock__dbSubblock : forall S TD Ps lc als gl Mem0 c lc1 als1 gl1 Mem1 tr1 cs lc2 als2 gl2 Mem2 tr2,
+  SimpleSE.dbCmd TD lc als gl Mem0 c lc1 als1 gl1 Mem1 tr1 ->
+  SimpleSE.dbSubblock S TD Ps lc1 als1 gl1 Mem1 cs lc2 als2 gl2 Mem2 tr2 ->
+  SimpleSE.dbSubblock S TD Ps lc als gl Mem0 (c::cs) lc2 als2 gl2 Mem2 (trace_app tr1 tr2).
+Proof.
+  intros S TD Ps lc als gl Mem0 c lc1 als1 gl1 Mem1 tr1 cs lc2 als2 gl2 Mem2 tr2 H1 H2.
+  inversion H2; subst.  
+  rewrite trace_app_commute.
+  assert (c::cs0++call0::nil = (c::cs0)++call0::nil) as EQ. auto.
+  rewrite EQ.
+  eapply SimpleSE.dbSubblock_intro; eauto.
+Qed.
+
+Lemma dbCmd_dbSubblocks__dbCmd_or_dbSubblocks : forall S TD Ps lc als gl Mem0 c lc1 als1 gl1 Mem1 tr1 cs lc2 als2 gl2 Mem2 tr2,
+  SimpleSE.dbCmd TD lc als gl Mem0 c lc1 als1 gl1 Mem1 tr1 ->
+  SimpleSE.dbSubblocks S TD Ps lc1 als1 gl1 Mem1 cs lc2 als2 gl2 Mem2 tr2 ->
+  (SimpleSE.dbCmd TD lc als gl Mem0 c lc2 als2 gl2 Mem2 tr1 /\ 
+   cs = nil /\ tr2 = trace_nil /\ 
+   lc1 = lc2 /\ als1 = als2 /\ gl1 = gl2 /\ Mem1 = Mem2 
+  ) \/
+  (SimpleSE.dbSubblocks S TD Ps lc als gl Mem0 (c::cs) lc2 als2 gl2 Mem2 (trace_app tr1 tr2)).
+Proof.
+  intros S TD Ps lc als gl Mem0 c lc1 als1 gl1 Mem1 tr1 cs lc2 als2 gl2 Mem2 tr2 H1 H2.
+  inversion H2; subst.
+    left. repeat (split; auto).
+    right. 
+      rewrite trace_app_commute.
+      assert (c::cs0++cs'=(c::cs0)++cs') as EQ. auto.
+      rewrite EQ.
+      eapply SimpleSE.dbSubblocks_cons; eauto using dbCmd_dbSubblock__dbSubblock.
+Qed.
+
+Lemma dbInsn__inv : forall S1 TD1 Ps1 F1 l1 ps1 cs1 tmn1 c cs tmn3 lc1 arg1 als1 ECs1 gl1 Mem1
+                         S2 TD2 Ps2 F2 l2 ps2 cs2 tmn2 tmn4 lc2 arg2 als2 ECs2 gl2 Mem2 tr,
+  dbInsn 
+    (mkState S1 TD1 Ps1 (mkEC F1 (block_intro l1 ps1 cs1 tmn1) (c::cs) tmn3 lc1 arg1 als1::ECs1) gl1 Mem1) 
+    (mkState S2 TD2 Ps2 (mkEC F2 (block_intro l2 ps2 cs2 tmn2) cs tmn4 lc2 arg2 als2::ECs2) gl2 Mem2)
+    tr ->
+  S1 = S2 /\ TD1 = TD2 /\ Ps1 = Ps2 /\ F1 = F2 /\ l1 = l2 /\ ps1 = ps2 /\
+  cs1 = cs2 /\ tmn1 = tmn2 /\ tmn3 = tmn4.
+Proof.
+  intros.
+  inversion H; subst; repeat (split; auto).
+Qed.
+
+
+Lemma dbTerminator_test : forall TD F l1 ps1 cs1 tmn1 lc1 gl1 B lc2 tr cs2,
+  SimpleSE.dbTerminator TD F (block_intro l1 ps1 cs1 tmn1) lc1 gl1 tmn1 B lc2 tr ->
+  SimpleSE.dbTerminator TD F (block_intro l1 ps1 cs2 tmn1) lc1 gl1 tmn1 B lc2 tr.
+Proof.
+  intros.
+  inversion H; subst. clear H.
+    eapply SimpleSE.dbBranch; eauto.
+       admit. (*block*)
+    eapply SimpleSE.dbBranch_uncond; eauto.
+       admit. (*block*)
+Qed.
+
+Lemma dbCmd_dbBlock__dbBlock : forall S TD Ps lc als gl Mem0 c lc1 als1 gl1 Mem1 tr1 lc2 als2 gl2 Mem2 tr2 
+  l1 ps1 cs1 tmn1 B F arg,
+  SimpleSE.dbCmd TD lc als gl Mem0 c lc1 als1 gl1 Mem1 tr1 ->
+  SimpleSE.dbBlock S TD Ps F arg 
+    (SimpleSE.mkState (SimpleSE.mkEC (block_intro l1 ps1 cs1 tmn1) lc1 als1) gl1 Mem1)
+    (SimpleSE.mkState (SimpleSE.mkEC B lc2 als2) gl2 Mem2)
+    tr2 ->
+  SimpleSE.dbBlock S TD Ps F arg 
+    (SimpleSE.mkState (SimpleSE.mkEC (block_intro l1 ps1 (c::cs1) tmn1) lc als) gl Mem0)
+    (SimpleSE.mkState (SimpleSE.mkEC B lc2 als2) gl2 Mem2)
+    (trace_app tr1 tr2).
+Proof.
+  intros S TD Ps lc als gl Mem0 c lc1 als1 gl1 Mem1 tr1 lc2 als2 gl2 Mem2 tr2 
+    l1 ps1 cs1 tmn1 B F arg0 H1 H2.
+  inversion H2; subst.  
+  rewrite trace_app_commute.
+  rewrite trace_app_commute.
+  apply dbCmd_dbSubblocks__dbCmd_or_dbSubblocks with (lc:=lc)(als:=als)(gl:=gl)(Mem0:=Mem0)(c:=c)(tr1:=tr1) in H20; auto.
+  destruct H20 as [[J11 [EQ [EQ' [EQ1 [EQ2 [EQ3 EQ4]]]]]] | J11]; subst.
+    assert (c::nil++cs'=nil++c::cs') as EQ. auto.
+    rewrite EQ. clear EQ.
+    rewrite trace_app_nil__eq__trace.
+    rewrite <- nil_app_trace__eq__trace.
+    rewrite trace_app_commute.
+    eapply SimpleSE.dbBlock_intro; eauto using dbTerminator_test.
+
+    assert (c::cs++cs'=(c::cs)++cs') as EQ. auto.
+    rewrite EQ. clear EQ.
+    eapply SimpleSE.dbBlock_intro; eauto using dbTerminator_test.
+Qed.
+
+
+Lemma dbCmd_dbBlocks__dbCmd_or_dbBlocks : forall S TD Ps lc als gl Mem0 c lc1 als1 gl1 Mem1 tr1 lc2 als2 gl2 Mem2 tr2 
+  l1 ps1 cs1 tmn1 l2 ps2 cs2 tmn2 F arg,
+  SimpleSE.dbCmd TD lc als gl Mem0 c lc1 als1 gl1 Mem1 tr1 ->
+  SimpleSE.dbBlocks S TD Ps F arg 
+    (SimpleSE.mkState (SimpleSE.mkEC (block_intro l1 ps1 cs1 tmn1) lc1 als1) gl1 Mem1)
+    (SimpleSE.mkState (SimpleSE.mkEC (block_intro l2 ps2 cs2 tmn2) lc2 als2) gl2 Mem2)
+    tr2 ->
+  (SimpleSE.dbCmd TD lc als gl Mem0 c lc2 als2 gl2 Mem2 tr1 /\ 
+   cs1 = cs2 /\ tr2 = trace_nil /\ 
+   lc1 = lc2 /\ als1 = als2 /\ gl1 = gl2 /\ Mem1 = Mem2 /\
+   l1 = l2 /\ ps1 = ps2 /\ tmn1 = tmn2
+  ) \/
+  (SimpleSE.dbBlocks S TD Ps F arg 
+    (SimpleSE.mkState (SimpleSE.mkEC (block_intro l1 ps1 (c::cs1) tmn1) lc als) gl Mem0)
+    (SimpleSE.mkState (SimpleSE.mkEC (block_intro l2 ps2 cs2 tmn2) lc2 als2) gl2 Mem2)
+    (trace_app tr1 tr2)).
+Proof.
+  intros S TD Ps lc als gl Mem0 c lc1 als1 gl1 Mem1 tr1 lc2 als2 gl2 Mem2 tr2 
+    l1 ps1 cs1 tmn1 l2 ps2 cs2 tmn2 F arg0 H1 H2.
+  inversion H2; subst.
+    left. repeat (split; auto).
+    right. 
+      rewrite trace_app_commute.
+      inversion H; subst.
+      eapply SimpleSE.dbBlocks_cons; eauto using dbCmd_dbBlock__dbBlock.
+Qed.
+
+
+Lemma dbCall__dbSubblock : forall S TD Ps lc gl Mem c lc' gl' Mem' tr als,
+  SimpleSE.dbCall S TD Ps lc gl Mem c lc' gl' Mem' tr ->
+  SimpleSE.dbSubblock S TD Ps 
+    lc als gl Mem
+    (c::nil)
+    lc' als gl' Mem'
+    tr.
+Proof.
+  intros S TD Ps lc gl Mem0 c lc' gl' Mem' tr als H.
+  rewrite <- nil_app_trace__eq__trace.
+  assert (c::nil=nil++c::nil) as EQ. auto.
+  rewrite EQ.
+  apply SimpleSE.dbSubblock_intro with (lc2:=lc)(gl2:=gl)(Mem2:=Mem0); auto.
+Qed.
+
+Lemma dbCall_isCallInst : forall S TD Ps lc gl Mem c lc' gl' Mem' tr,
+  SimpleSE.dbCall S TD Ps lc gl Mem c lc' gl' Mem' tr ->
+  Instruction.isCallInst c = true.
+Proof.
+  intros S TD Ps lc gl Mem0 c lc' gl' Mem' tr HdbCall.
+  induction HdbCall; auto.
+Qed.
+
+Lemma dbInsn_Call__inv : forall S1 TD1 Ps1 F1 l1 ps1 cs1 tmn1 c cs tmn3 lc1 arg1 als1 ECs1 gl1 Mem1
+                         S2 TD2 Ps2 F2 l2 ps2 cs2 tmn2 tmn4 lc2 arg2 als2 ECs2 gl2 Mem2 tr,
+  
+  dbInsn 
+    (mkState S1 TD1 Ps1 (mkEC F1 (block_intro l1 ps1 cs1 tmn1) (c::cs) tmn3 lc1 arg1 als1::ECs1) gl1 Mem1) 
+    (mkState S2 TD2 Ps2 (mkEC F2 (block_intro l2 ps2 cs2 tmn2) cs tmn4 lc2 arg2 als2::ECs2) gl2 Mem2)
+    tr ->
+  Instruction.isCallInst c = true ->
+  S1 = S2 /\ TD1 = TD2 /\ Ps1 = Ps2 /\ F1 = F2 /\ l1 = l2 /\ ps1 = ps2 /\
+  cs1 = cs2 /\ tmn1 = tmn2 /\ tmn3 = tmn4 /\ als1 = als2.
+Proof.
+  intros.
+  inversion H; subst; try solve [inversion H0].
+    repeat (split; auto).
+Qed.
+
+Lemma dbSubblock_dbBlock__dbBlock : forall S TD Ps lc als gl Mem0 cs lc1 als1 gl1 Mem1 tr1 lc2 als2 gl2 Mem2 tr2 
+  l1 ps1 cs1 tmn1 B F arg,
+  SimpleSE.dbSubblock S TD Ps lc als gl Mem0 cs lc1 als1 gl1 Mem1 tr1 ->
+  SimpleSE.dbBlock S TD Ps F arg 
+    (SimpleSE.mkState (SimpleSE.mkEC (block_intro l1 ps1 cs1 tmn1) lc1 als1) gl1 Mem1)
+    (SimpleSE.mkState (SimpleSE.mkEC B lc2 als2) gl2 Mem2)
+    tr2 ->
+  SimpleSE.dbBlock S TD Ps F arg 
+    (SimpleSE.mkState (SimpleSE.mkEC (block_intro l1 ps1 (cs++cs1) tmn1) lc als) gl Mem0)
+    (SimpleSE.mkState (SimpleSE.mkEC B lc2 als2) gl2 Mem2)
+    (trace_app tr1 tr2).
+Proof.
+  intros S TD Ps lc als gl Mem0 cs lc1 als1 gl1 Mem1 tr1 lc2 als2 gl2 Mem2 tr2 
+    l1 ps1 cs1 tmn1 B F arg0 H1 H2.
+  inversion H2; subst.  
+  rewrite trace_app_commute.
+  rewrite trace_app_commute.
+  rewrite <- app_ass.
+  eapply SimpleSE.dbBlock_intro; eauto using dbTerminator_test.
+Qed.
+
+Lemma dbSubblock_dbBlocks__dbSubblock_or_dbBlocks : forall S TD Ps lc als gl Mem0 cs lc1 als1 gl1 Mem1 tr1 lc2 als2 gl2 Mem2 tr2 
+  l1 ps1 cs1 tmn1 l2 ps2 cs2 tmn2 F arg,
+  SimpleSE.dbSubblock S TD Ps lc als gl Mem0 cs lc1 als1 gl1 Mem1 tr1 ->
+  SimpleSE.dbBlocks S TD Ps F arg 
+    (SimpleSE.mkState (SimpleSE.mkEC (block_intro l1 ps1 cs1 tmn1) lc1 als1) gl1 Mem1)
+    (SimpleSE.mkState (SimpleSE.mkEC (block_intro l2 ps2 cs2 tmn2) lc2 als2) gl2 Mem2)
+    tr2 ->
+  (  SimpleSE.dbSubblock S TD Ps lc als gl Mem0 cs lc1 als1 gl1 Mem1 tr1 /\ 
+   cs1 = cs2 /\ tr2 = trace_nil /\ 
+   lc1 = lc2 /\ als1 = als2 /\ gl1 = gl2 /\ Mem1 = Mem2 /\
+   l1 = l2 /\ ps1 = ps2 /\ tmn1 = tmn2
+  ) \/
+  (SimpleSE.dbBlocks S TD Ps F arg 
+    (SimpleSE.mkState (SimpleSE.mkEC (block_intro l1 ps1 (cs++cs1) tmn1) lc als) gl Mem0)
+    (SimpleSE.mkState (SimpleSE.mkEC (block_intro l2 ps2 cs2 tmn2) lc2 als2) gl2 Mem2)
+    (trace_app tr1 tr2)).
+Proof.
+  intros S TD Ps lc als gl Mem0 cs lc1 als1 gl1 Mem1 tr1 lc2 als2 gl2 Mem2 tr2 
+    l1 ps1 cs1 tmn1 l2 ps2 cs2 tmn2 F arg0 H1 H2.
+  inversion H2; subst.
+    left. repeat (split; auto).
+    right. 
+      rewrite trace_app_commute.
+      inversion H; subst.
+      eapply SimpleSE.dbBlocks_cons; eauto using dbSubblock_dbBlock__dbBlock.
+Qed.
+
+
+Definition llvmop_dbInsn__seop_prop state1 state2 tr
+  (db:LLVMopsem.dbInsn state1 state2 tr) :=
+  forall S TD Ps F l ps cs tmn lc arg als ECs gl Mem cs0,
+  state1 = (mkState S TD Ps ((mkEC F (block_intro l ps cs0 tmn) cs tmn lc arg als)::ECs) gl Mem) ->
+  exists l', exists ps', exists cs', exists tmn', 
+  exists lc', exists als', exists gl', exists Mem', exists cs0',
+  state2 = (mkState S TD Ps ((mkEC F (block_intro l' ps' cs0' tmn') cs' tmn' lc' arg als')::ECs) gl' Mem') /\
+  ((cs = nil /\ Mem = Mem' /\ als = als' /\ gl = gl' /\ cs' = cs0' /\
+              SimpleSE.dbTerminator TD F 
+                 (block_intro l ps cs tmn) lc gl 
+                 tmn 
+                 (block_intro l' ps' cs' tmn') lc' 
+                 tr ) \/ 
+  (exists c, c::cs' = cs /\ SimpleSE.dbCmd TD lc als gl Mem c lc' als' gl' Mem' tr) \/
+  (exists c, c::cs' = cs /\ SimpleSE.dbCall S TD Ps lc gl Mem c lc' gl' Mem' tr)).
+Definition llvmop_dbop__seop_prop state1 state2 tr
+  (db:LLVMopsem.dbop state1 state2 tr) :=
+  forall S TD Ps F l ps cs tmn lc arg als ECs gl Mem l' ps' cs' tmn' lc' als' gl' Mem' cs0 cs0',
+  state1 = (mkState S TD Ps ((mkEC F (block_intro l ps cs0 tmn) cs tmn lc arg als)::ECs) gl Mem) ->
+  state2 = (mkState S TD Ps ((mkEC F (block_intro l' ps' cs0' tmn') cs' tmn' lc' arg als')::ECs) gl' Mem') ->
+  (exists cs1, exists cs2, 
+  exists tr1, exists tr2,
+  exists lc1, exists als1, exists gl1, exists Mem1,
+    trace_app tr1 tr2 = tr /\  
+    l = l' /\
+    ps = ps' /\
+    cs0 = cs0' /\
+    tmn = tmn' /\
+    cs = cs1++cs2++cs' /\
+    SimpleSE.dbSubblocks S TD Ps
+      lc als gl Mem
+      cs1
+      lc1 als1 gl1 Mem1
+      tr1 /\
+    SimpleSE.dbCmds TD
+      lc1 als1 gl1 Mem1
+      cs2
+      lc' als' gl' Mem'
+      tr2) \/
+  (exists cs1, exists cs2, 
+  exists tr1, exists tr2, exists tr3,
+  exists lc1, exists als1, exists gl1, exists Mem1,
+  exists lc2, exists als2, exists gl2, exists Mem2,
+    cs1++cs2++cs'=cs0' /\
+    (trace_app (trace_app tr1 tr2) tr3) = tr /\
+    SimpleSE.dbBlocks S TD Ps F arg 
+      (SimpleSE.mkState (SimpleSE.mkEC (block_intro l ps cs tmn) lc als) gl Mem) 
+      (SimpleSE.mkState (SimpleSE.mkEC (block_intro l' ps' cs0' tmn') lc1 als1) gl1 Mem1)
+      tr1 /\
+    SimpleSE.dbSubblocks S TD Ps
+      lc1 als1 gl1 Mem1
+      cs1
+      lc2 als2 gl2 Mem2
+      tr2 /\
+    SimpleSE.dbCmds TD
+      lc2 als2 gl2 Mem2
+      cs2
+      lc' als' gl' Mem'
+      tr3).
+Definition llvmop_dbFdef__seop_dbFdef_prop fid rt lp S TD Ps ECs lc gl Mem lc' gl' als' Mem' B' Rid oResult tr
+  (db:LLVMopsem.dbFdef fid rt lp S TD Ps ECs lc gl Mem lc' gl' als' Mem' B' Rid oResult tr) :=
+  SimpleSE.dbFdef fid rt lp S TD Ps lc gl Mem lc' gl' als' Mem' B' Rid oResult tr.
+
+Lemma llvmop__seop : 
+  (forall state1 state2 tr db, @llvmop_dbInsn__seop_prop state1 state2 tr db) /\
+  (forall state1 state2 tr db, @llvmop_dbop__seop_prop state1 state2 tr  db) /\
+  (forall fid rt lp S TD Ps lc gl Mem lc' gl' als' Mem' B' Rid oResult tr ECs db, 
+    @llvmop_dbFdef__seop_dbFdef_prop fid rt lp S TD Ps lc gl Mem lc' gl' als' Mem' B' Rid oResult tr ECs db).
+Proof.
+(db_mutind_cases
+  apply LLVMopsem.db_mutind with
+    (P  := llvmop_dbInsn__seop_prop)
+    (P0 := llvmop_dbop__seop_prop)
+    (P1 := llvmop_dbFdef__seop_dbFdef_prop) Case);
+  unfold llvmop_dbInsn__seop_prop, 
+         llvmop_dbop__seop_prop, 
+         llvmop_dbFdef__seop_dbFdef_prop; intros; subst.
+Case "dbBranch".
+  inversion H; subst. clear H.
+  exists l'. exists ps'. exists cs'. exists tmn'.
+  exists (switchToNewBasicBlock (block_intro l' ps' cs' tmn') (block_intro l0 ps cs0 (insn_br bid Cond l1 l2)) lc0). exists als0. exists gl0. exists Mem1.
+  exists cs'. split; auto.
+  left. 
+  split; auto.
+  split; auto.
+  split; auto.
+  split; auto.
+  split; auto.
+    apply SimpleSE.dbBranch with (c:=c); auto.
+      rewrite e0. admit. (*lookup*)
+      simpl. admit. (*switch*)
+
+Case "dbBranch_uncond".
+  inversion H; subst. clear H.
+  exists l'. exists ps'. exists cs'. exists tmn'.
+  exists (switchToNewBasicBlock (block_intro l' ps' cs' tmn') (block_intro l1 ps cs0 (insn_br_uncond bid l0)) lc0). exists als0. exists gl0. exists Mem1.
+  exists cs'. split; auto.
+  left.
+  split; auto.
+  split; auto.
+  split; auto.
+  split; auto.
+  split; auto.
+    apply SimpleSE.dbBranch_uncond; auto.
+      rewrite e. admit. (*lookup*)
+      simpl. admit. (*switch*)
+
+Case "dbBop".
+  inversion H; subst. clear H.
+  exists l0. exists ps. exists cs. exists tmn0.
+  exists lc'. exists als0. exists gl'. exists Mem1.
+  exists cs1. split; auto.
+  right. left.
+  exists (insn_bop id0 bop0 sz0 v1 v2).
+  split; eauto.
+
+Case "dbExtractValue".
+  inversion H; subst. clear H.
+  exists l0. exists ps. exists cs. exists tmn0.
+  exists lc'. exists als0. exists gl'. exists Mem1.
+  exists cs1. split; auto.
+  right. left.
+  exists (insn_extractvalue id0 t v idxs).
+  split; eauto.
+
+Case "dbInsertValue".
+  inversion H; subst. clear H.
+  exists l0. exists ps. exists cs. exists tmn0.
+  exists lc'. exists als0. exists gl'. exists Mem1.
+  exists cs1. split; auto.
+  right. left.
+  exists (insn_insertvalue id0 t v t' v' idxs).
+  split; eauto.
+
+Case "dbMalloc".
+  inversion H; subst. clear H. 
+  exists l0. exists ps. exists cs. exists tmn0.
+  exists lc'. exists als0. exists gl'. exists Mem'.
+  exists cs1. split; auto.
+  right. left.
+  exists (insn_malloc id0 t sz0 align0).
+  split; eauto.
+
+Case "dbFree".
+  inversion H; subst. clear H.
+  exists l0. exists ps. exists cs. exists tmn0.
+  exists lc0. exists als0. exists gl0. exists Mem'.
+  exists cs1. split; auto.
+  right. left.
+  exists (insn_free fid t v).
+  split; eauto.
+
+Case "dbAlloca".
+  inversion H; subst. clear H.
+  exists l0. exists ps. exists cs. exists tmn0.
+  exists lc'. exists (mb::als0). exists gl'. exists Mem'.
+  exists cs1. split; auto.
+  right. left.
+  exists (insn_alloca id0 t sz0 align0).
+  split; eauto.
+
+Case "dbLoad".
+  inversion H; subst. clear H.
+  exists l0. exists ps. exists cs. exists tmn0.
+  exists lc'. exists als0. exists gl'. exists Mem1.
+  exists cs1. split; auto.
+  right. left.
+  exists (insn_load id0 t v).
+  split; eauto.
+
+Case "dbStore".
+  inversion H; subst. clear H.
+  exists l0. exists ps. exists cs. exists tmn0.
+  exists lc0. exists als0. exists gl0. exists Mem'.
+  exists cs1. split; auto.
+  right. left.
+  exists (insn_store sid t v1 v2).
+  split; eauto.
+
+Case "dbGEP".
+  inversion H; subst. clear H.
+  exists l0. exists ps. exists cs. exists tmn0.
+  exists lc'. exists als0. exists gl'. exists Mem1.
+  exists cs1. split; auto.
+  right. left.
+  exists (insn_gep id0 inbounds0 t v idxs).
+  split; eauto.
+
+Case "dbExt".
+  inversion H; subst. clear H.
+  exists l0. exists ps. exists cs. exists tmn0.
+  exists lc'. exists als0. exists gl'. exists Mem1.
+  exists cs1. split; auto.
+  right. left.
+  exists (insn_ext id0 extop0 t1 v1 t2).
+  split; eauto.
+
+Case "dbCast".
+  inversion H; subst. clear H.
+  exists l0. exists ps. exists cs. exists tmn0.
+  exists lc'. exists als0. exists gl'. exists Mem1.
+  exists cs1. split; auto.
+  right. left.
+  exists (insn_cast id0 castop0 t1 v1 t2).
+  split; eauto.
+
+Case "dbIcmp".
+  inversion H; subst. clear H.
+  exists l0. exists ps. exists cs. exists tmn0.
+  exists lc'. exists als0. exists gl'. exists Mem1.
+  exists cs1. split; auto.
+  right. left.
+  exists (insn_icmp id0 cond0 t v1 v2).
+  split; eauto.
+
+Case "dbSelect".
+  inversion H; subst. clear H.
+  exists l0. exists ps. exists cs. exists tmn0.
+  exists lc'. exists als0. exists gl'. exists Mem1.
+  exists cs1. split; auto.
+  right. left.
+  exists (insn_select id0 v0 t v1 v2).
+  split; eauto.
+
+Case "dbCall".
+  inversion H0; subst. clear H0.
+  exists l0. exists ps. exists cs. exists tmn0.
+  exists lc''. exists als0. exists gl''. exists Mem''.
+  exists cs1. split; auto.
+  right. right.
+  exists (insn_call rid noret0 tailc0 rt fid lp).
+  split; eauto.
+
+Case "dbop_nil".
+  inversion H0; subst. clear H0. 
+  left.
+  exists nil. exists nil.
+  exists trace_nil. exists trace_nil.
+  exists lc'. exists als'. exists gl'. exists Mem'.
+  repeat (split; auto).
+  
+Case "dbop_cons".
+  destruct (@H S TD Ps F l0 ps cs tmn lc arg0 als ECs gl Mem0 cs0)
+    as [l1 [ps1 [cs1 [tmn1 [lc1 [als1 [gl1 [Mem1 [cs2 [J1 J2]]]]]]]]]]; subst; auto.
+  clear H.
+  assert (mkState S TD Ps (mkEC F (block_intro l1 ps1 cs2 tmn1) cs1 tmn1 lc1 arg0 als1::ECs) gl1 Mem1 =
+          mkState S TD Ps (mkEC F (block_intro l1 ps1 cs2 tmn1) cs1 tmn1 lc1 arg0 als1::ECs) gl1 Mem1) as J'. auto.
+  apply H0 with (l'0:=l')(ps'0:=ps')(cs'0:=cs')(tmn'0:=tmn')(lc'0:=lc')(als'0:=als')(gl'0:=gl')(Mem'0:=Mem')(cs0'0:=cs0') in J'; auto.
+  clear H0.
+  destruct J2 as [[EQ [EQ' [EQ1 [EQ2 [EQ3 J2]]]]] | [[c [EQ J2]] | [c [EQ J2]]]]; subst.
+  SCase "dbTerminator".
+    destruct J' as [
+                     [cs3 [cs4 [tr1 [tr2 [lc2 [als2 [gl2 [Mem2 [EQ1 [EQ2 [EQ3 [EQ4 [EQ5 [EQ6 [J11 J12]]]]]]]]]]]]]]] | 
+                     [cs3 [cs4 [tr1 [tr2 [tr3 [lc2 [als2 [gl2 [Mem2 [lc3 [als3 [gl3 [Mem3 [EQ1 [EQ2 [J21 [J22 J23]]]]]]]]]]]]]]]]]
+                   ]; subst.
+    SSCase "one block".
+      subst.
+      right.
+      exists cs3. exists cs4.
+      exists t1. exists tr1. exists tr2.
+      exists lc1. exists als1. exists gl1. exists Mem1.
+      exists lc2. exists als2. exists gl2. exists Mem2.
+      rewrite trace_app_commute.
+      repeat (split; auto).
+        apply dbBlock__dbBlocks; auto using dbTerminator__dbBlock.
+    
+    SSCase "multi block".
+      right.
+      exists cs3. exists cs4.
+      exists (trace_app t1 tr1). exists tr2. exists tr3.
+      exists lc2. exists als2. exists gl2. exists Mem2.
+      exists lc3. exists als3. exists gl3. exists Mem3.
+      rewrite trace_app_commute.
+      rewrite trace_app_commute.
+      repeat (split; auto).
+        apply SimpleSE.dbBlocks_cons with (S2:=SimpleSE.mkState (SimpleSE.mkEC (block_intro l1 ps1 cs2 tmn1) lc1 als1) gl1 Mem1); 
+          auto using dbTerminator__dbBlock.
+  SCase "dbCmd".
+    apply dbInsn__inv in d.
+    destruct d as [_ [_ [_ [_ [EQ5 [EQ6 [EQ7 [EQ8 _]]]]]]]]; subst.
+    destruct J' as [
+                     [cs3 [cs4 [tr1 [tr2 [lc2 [als2 [gl2 [Mem2 [EQ1 [EQ2 [EQ3 [EQ4 [EQ5 [EQ6 [J11 J12]]]]]]]]]]]]]]] | 
+                     [cs3 [cs4 [tr1 [tr2 [tr3 [lc2 [als2 [gl2 [Mem2 [lc3 [als3 [gl3 [Mem3 [EQ1 [EQ2 [J21 [J22 J23]]]]]]]]]]]]]]]]]
+                   ]; subst.
+    SSCase "one block".
+      left.
+      apply dbCmd_dbSubblocks__dbCmd_or_dbSubblocks with (lc:=lc)(als:=als)(gl:=gl)(Mem0:=Mem0)(c:=c)(tr1:=t1) in J11; auto.
+      destruct J11 as [[J11 [EQ [EQ' [EQ1 [EQ2 [EQ3 EQ4]]]]]] | J11]; subst.
+        exists nil. exists (c::cs4).
+        exists trace_nil. exists (trace_app t1 tr2).
+        exists lc. exists als. exists gl. exists Mem0.
+        rewrite nil_app_trace__eq__trace.
+        rewrite nil_app_trace__eq__trace.
+        repeat (split; eauto). 
+
+        exists (c::cs3). exists cs4.
+        exists (trace_app t1 tr1). exists tr2.
+        exists lc2. exists als2. exists gl2. exists Mem2.
+        rewrite trace_app_commute. simpl_env in *.
+        repeat (split; auto).
+    
+    SSCase "multi block".
+      apply dbCmd_dbBlocks__dbCmd_or_dbBlocks with (lc:=lc)(als:=als)(gl:=gl)(Mem0:=Mem0)(c:=c)(tr1:=t1) in J21; auto.
+      destruct J21 as [[J21 [EQ [EQ' [EQ1 [EQ2 [EQ3 [EQ4 [EQ5 [EQ6 EQ7]]]]]]]]] | J21]; subst.
+        apply dbCmd_dbSubblocks__dbCmd_or_dbSubblocks with (lc:=lc)(als:=als)(gl:=gl)(Mem0:=Mem0)(c:=c)(tr1:=t1) in J22; auto.
+        destruct J22 as [[J22 [EQ [EQ' [EQ1 [EQ2 [EQ3 EQ4]]]]]] | J22]; subst.
+          left. 
+          exists nil. exists (c::cs4).
+          exists trace_nil. exists (trace_app t1 tr3).
+          exists lc. exists als. exists gl. exists Mem0.
+          rewrite nil_app_trace__eq__trace.
+          rewrite nil_app_trace__eq__trace.
+          repeat (split; eauto).
+            admit. (*block*) 
+      
+          left.
+          exists (c::cs3). exists cs4.
+          exists (trace_app t1 tr2). exists tr3.
+          exists lc3. exists als3. exists gl3. exists Mem3.
+          rewrite nil_app_trace__eq__trace.
+          rewrite trace_app_commute.
+          repeat (split; eauto).
+            admit. (*block*) 
+        
+        right.
+        exists cs3. exists cs4.
+        exists (trace_app t1 tr1). exists tr2. exists tr3.
+        exists lc2. exists als2. exists gl2. exists Mem2.
+        exists lc3. exists als3. exists gl3. exists Mem3.
+        rewrite trace_app_commute.
+        rewrite trace_app_commute.
+        repeat (split; eauto).
+
+  SCase "dbCall".
+    assert (J:=J2).
+    apply dbCall_isCallInst in J.
+    apply dbCall__dbSubblock with (als:=als1) in J2.
+    apply dbInsn_Call__inv in d; auto.
+    destruct d as [_ [_ [_ [_ [EQ5 [EQ6 [EQ7 [EQ8 [_ EQ9]]]]]]]]]; subst.
+    destruct J' as [
+                     [cs3 [cs4 [tr1 [tr2 [lc2 [als2 [gl2 [Mem2 [EQ1 [EQ2 [EQ3 [EQ4 [EQ5 [EQ6 [J11 J12]]]]]]]]]]]]]]] | 
+                     [cs3 [cs4 [tr1 [tr2 [tr3 [lc2 [als2 [gl2 [Mem2 [lc3 [als3 [gl3 [Mem3 [EQ1 [EQ2 [J21 [J22 J23]]]]]]]]]]]]]]]]]
+                   ]; subst.
+    SSCase "one block".
+      left.
+      exists (c::cs3). exists cs4.
+      exists (trace_app t1 tr1). exists tr2.
+      exists lc2. exists als2. exists gl2. exists Mem2.
+      rewrite trace_app_commute. simpl_env in *.
+      repeat (split; eauto).
+
+    SSCase "multi block".
+      apply dbSubblock_dbBlocks__dbSubblock_or_dbBlocks with (lc:=lc)(als:=als1)(gl:=gl)(Mem0:=Mem0)(cs:=c::nil)(tr1:=t1) in J21; auto.
+      destruct J21 as [[J21 [EQ [EQ' [EQ1 [EQ2 [EQ3 [EQ4 [EQ5 [EQ6 EQ7]]]]]]]]] | J21]; subst.
+        left. 
+        exists (c::cs3). exists cs4.
+        exists (trace_app t1 tr2). exists tr3.
+        exists lc3. exists als3. exists gl3. exists Mem3.
+        rewrite nil_app_trace__eq__trace.
+        rewrite trace_app_commute. simpl_env in *.
+        repeat (split; eauto).
+          admit. (*block*) 
+      
+        right.
+        exists cs3. exists cs4.
+        exists (trace_app t1 tr1). exists tr2. exists tr3.
+        exists lc2. exists als2. exists gl2. exists Mem2.
+        exists lc3. exists als3. exists gl3. exists Mem3.
+        rewrite trace_app_commute.
+        rewrite trace_app_commute.
+        repeat (split; eauto).     
+
+Case "dbFdef_func".
+  assert (mkState S TD Ps (mkEC (fdef_intro (fheader_intro rt fid la) lb) (block_intro l' ps' cs' tmn') cs' tmn' (initLocals la (params2GVs TD lp lc gl)) (params2GVs TD lp lc gl) nil::ECs) gl Mem0 =
+          mkState S TD Ps (mkEC (fdef_intro (fheader_intro rt fid la) lb) (block_intro l' ps' cs' tmn') cs' tmn' (initLocals la (params2GVs TD lp lc gl)) (params2GVs TD lp lc gl) nil::ECs) gl Mem0) as J. auto.
+  apply H with (l'0:=l'')(ps'0:=ps'')(cs'0:=nil)(tmn'0:=insn_return rid rt Result)(lc'0:=lc')(als'0:=als')(gl'0:=gl')(Mem'0:=Mem')(cs0':=cs'') in J; auto.
+  clear H d.
+  destruct J as [
+                 [cs3 [cs4 [tr1 [tr2 [lc2 [als2 [gl2 [Mem2 [EQ1 [EQ2 [EQ3 [EQ4 [EQ5 [EQ6 [J11 J12]]]]]]]]]]]]]]] | 
+                 [cs3 [cs4 [tr1 [tr2 [tr3 [lc2 [als2 [gl2 [Mem2 [lc3 [als3 [gl3 [Mem3 [EQ1 [EQ2 [J21 [J22 J23]]]]]]]]]]]]]]]]]
+                ]; subst.
+  SCase "one block".
+    simpl_env in EQ6. subst.
+    rewrite <- nil_app_trace__eq__trace with (tr:=tr1).
+    eapply SimpleSE.dbFdef_func; eauto.
+      rewrite <- e. 
+      admit. (*lookup*)
+  
+  SCase "multi block".
+    simpl_env in *.
+    eapply SimpleSE.dbFdef_func; eauto.
+      rewrite <- e. 
+      admit. (*lookup*)
+
+Case "dbFdef_proc".
+  assert (mkState S TD Ps (mkEC (fdef_intro (fheader_intro rt fid la) lb) (block_intro l' ps' cs' tmn') cs' tmn' (initLocals la (params2GVs TD lp lc gl)) (params2GVs TD lp lc gl) nil::ECs) gl Mem0 =
+          mkState S TD Ps (mkEC (fdef_intro (fheader_intro rt fid la) lb) (block_intro l' ps' cs' tmn') cs' tmn' (initLocals la (params2GVs TD lp lc gl)) (params2GVs TD lp lc gl) nil::ECs) gl Mem0) as J. auto.
+  apply H with (l'0:=l'')(ps'0:=ps'')(cs'0:=nil)(tmn'0:=insn_return_void rid)(lc'0:=lc')(als'0:=als')(gl'0:=gl')(Mem'0:=Mem')(cs0':=cs'') in J; auto.
+  clear H d.
+  destruct J as [
+                 [cs3 [cs4 [tr1 [tr2 [lc2 [als2 [gl2 [Mem2 [EQ1 [EQ2 [EQ3 [EQ4 [EQ5 [EQ6 [J11 J12]]]]]]]]]]]]]]] | 
+                 [cs3 [cs4 [tr1 [tr2 [tr3 [lc2 [als2 [gl2 [Mem2 [lc3 [als3 [gl3 [Mem3 [EQ1 [EQ2 [J21 [J22 J23]]]]]]]]]]]]]]]]]
+                ]; subst.
+  SCase "one block".
+    simpl_env in EQ6. subst.
+    rewrite <- nil_app_trace__eq__trace with (tr:=tr1).
+    eapply SimpleSE.dbFdef_proc; eauto.
+      rewrite <- e. 
+      admit. (*lookup*)
+  
+  SCase "multi block".
+    simpl_env in *.
+    eapply SimpleSE.dbFdef_proc; eauto.
+      rewrite <- e. 
+      admit. (*lookup*)
+Qed.
+
+
+Lemma llvmop_dbInsn__seop : forall state2 tr S TD Ps F l ps cs tmn lc arg als ECs gl Mem cs0,
+  LLVMopsem.dbInsn 
+    (mkState S TD Ps ((mkEC F (block_intro l ps cs0 tmn) cs tmn lc arg als)::ECs) gl Mem)  
+    state2 
+    tr ->
+  exists l', exists ps', exists cs', exists tmn', 
+  exists lc', exists als', exists gl', exists Mem', exists cs0',
+  state2 = (mkState S TD Ps ((mkEC F (block_intro l' ps' cs0' tmn') cs' tmn' lc' arg als')::ECs) gl' Mem') /\
+  ((cs = nil /\ Mem = Mem' /\ als = als' /\ gl = gl' /\ cs' = cs0' /\
+              SimpleSE.dbTerminator TD F 
+                 (block_intro l ps cs tmn) lc gl 
+                 tmn 
+                 (block_intro l' ps' cs' tmn') lc' 
+                 tr ) \/ 
+  (exists c, c::cs' = cs /\ SimpleSE.dbCmd TD lc als gl Mem c lc' als' gl' Mem' tr) \/
+  (exists c, c::cs' = cs /\ SimpleSE.dbCall S TD Ps lc gl Mem c lc' gl' Mem' tr)).
+Proof.
+  intros.
+  destruct llvmop__seop as [J _]. 
+  unfold llvmop_dbInsn__seop_prop in J.
+  eapply J; eauto.
+Qed.
+
+Lemma llvmop_dbop__seop : forall tr S TD Ps F l ps cs tmn lc arg als ECs gl Mem l' ps' cs' tmn' lc' als' gl' Mem' cs0 cs0',
+  LLVMopsem.dbop 
+    (mkState S TD Ps ((mkEC F (block_intro l ps cs0 tmn) cs tmn lc arg als)::ECs) gl Mem)
+    (mkState S TD Ps ((mkEC F (block_intro l' ps' cs0' tmn') cs' tmn' lc' arg als')::ECs) gl' Mem')
+    tr ->
+  (exists cs1, exists cs2, 
+  exists tr1, exists tr2,
+  exists lc1, exists als1, exists gl1, exists Mem1,
+    trace_app tr1 tr2 = tr /\  
+    l = l' /\
+    ps = ps' /\
+    cs0 = cs0' /\
+    tmn = tmn' /\
+    cs = cs1++cs2++cs' /\
+    SimpleSE.dbSubblocks S TD Ps
+      lc als gl Mem
+      cs1
+      lc1 als1 gl1 Mem1
+      tr1 /\
+    SimpleSE.dbCmds TD
+      lc1 als1 gl1 Mem1
+      cs2
+      lc' als' gl' Mem'
+      tr2) \/
+  (exists cs1, exists cs2, 
+  exists tr1, exists tr2, exists tr3,
+  exists lc1, exists als1, exists gl1, exists Mem1,
+  exists lc2, exists als2, exists gl2, exists Mem2,
+    cs1++cs2++cs'=cs0' /\
+    (trace_app (trace_app tr1 tr2) tr3) = tr /\
+    SimpleSE.dbBlocks S TD Ps F arg 
+      (SimpleSE.mkState (SimpleSE.mkEC (block_intro l ps cs tmn) lc als) gl Mem) 
+      (SimpleSE.mkState (SimpleSE.mkEC (block_intro l' ps' cs0' tmn') lc1 als1) gl1 Mem1)
+      tr1 /\
+    SimpleSE.dbSubblocks S TD Ps
+      lc1 als1 gl1 Mem1
+      cs1
+      lc2 als2 gl2 Mem2
+      tr2 /\
+    SimpleSE.dbCmds TD
+      lc2 als2 gl2 Mem2
+      cs2
+      lc' als' gl' Mem'
+      tr3).
+Proof.
+  intros.
+  destruct llvmop__seop as [_ [J _]]. 
+  unfold llvmop_dbop__seop_prop in J.
+  eapply J; eauto.
+Qed.
+
+Lemma llvmop_dbFdef__seop_dbFdef : forall fid rt lp S TD Ps ECs lc gl Mem lc' gl' als' Mem' B' Rid oResult tr,
+  LLVMopsem.dbFdef fid rt lp S TD Ps ECs lc gl Mem lc' gl' als' Mem' B' Rid oResult tr ->
+  SimpleSE.dbFdef fid rt lp S TD Ps lc gl Mem lc' gl' als' Mem' B' Rid oResult tr.
+Proof.
+  intros.
+  destruct llvmop__seop as [_ [_ J]]. 
+  unfold llvmop_dbFdef__seop_dbFdef_prop in J.
+  eapply J; eauto.
+Qed.
+
+
+
